ConcreteImmutability.v
@@ -514,7 +514,7 @@ Proof.
         simpl.
         destruct (nth_error vals i') as [v|] eqn:Hval_i.
           - (* Parameter i' exists *)
-            destruct v as [|loc]; [trivial|].
+            destruct v as [|loc|n]; [trivial| | trivial].
             (* Use Hrcv_sub to get the subtyping relationship *)
             assert (Hi'_bound : i' < List.length argtypes).
             {
@@ -545,6 +545,7 @@ Proof.
                       | Some _ => True
                       | None => False
                       end
+                  | Int _ => True
                   end) vals).
               {
                 eapply runtime_lookup_list_preserves_wf_values; eauto.
@@ -1371,7 +1372,7 @@ Proof.
         simpl.
         destruct (nth_error vals i') as [v|] eqn:Hval_i.
           - (* Parameter i' exists *)
-            destruct v as [|loc]; [trivial|].
+            destruct v as [|loc|n]; [trivial| | trivial].
             (* Use Hrcv_sub to get the subtyping relationship *)
             assert (Hi'_bound : i' < List.length argtypes).
             {
@@ -1402,6 +1403,7 @@ Proof.
                       | Some _ => True
                       | None => False
                       end
+                  | Int _ => True
                   end) vals).
               {
                 eapply runtime_lookup_list_preserves_wf_values; eauto.
@@ -2299,7 +2301,7 @@ Proof.
         simpl.
         destruct (nth_error vals i') as [v|] eqn:Hval_i.
           - (* Parameter i' exists *)
-            destruct v as [|loc]; [trivial|].
+            destruct v as [|loc|n]; [trivial| | trivial].
             assert (Hi'_bound : i' < List.length argtypes).
             {
               apply Forall2_length in Harg_sub.
@@ -2329,6 +2331,7 @@ Proof.
                       | Some _ => True
                       | None => False
                       end
+                  | Int _ => True
                   end) vals).
               {
                 eapply runtime_lookup_list_preserves_wf_values; eauto.
@@ -2967,7 +2970,7 @@ Proof.
         simpl.
         destruct (nth_error vals i') as [v|] eqn:Hval_i.
           - (* Parameter i' exists *)
-            destruct v as [|loc]; [trivial|].
+            destruct v as [|loc|n]; [trivial| | trivial].
             (* Use Hrcv_sub to get the subtyping relationship *)
             assert (Hi'_bound : i' < List.length argtypes).
             {
@@ -2998,6 +3001,7 @@ Proof.
                       | Some _ => True
                       | None => False
                       end
+                  | Int _ => True
                   end) vals).
               {
                 eapply runtime_lookup_list_preserves_wf_values; eauto.
