ConcurrentPico.v
@@ -1,0 +1,244 @@
+Require Import Syntax Helpers Typing Bigstep DerivedCache.
+
+From Stdlib Require Import List Lia.
+Import ListNotations.
+
+(* A first concurrent PICO machine.
+
+   This is intentionally smaller than Java's full memory model.  It is an
+   interleaving semantics with one shared heap and one runtime environment plus
+   residual statement per thread.  Heap updates are ordinary sequentially
+   consistent steps.  This gives us a real concurrent PICO artifact to connect
+   to the derived-cache invariant before adding weak-memory features.
+*)
+
+Record thread_state := mkThread {
+  thread_env : r_env;
+  thread_stmt : stmt;
+}.
+
+Record concurrent_config := mkConcurrentConfig {
+  concurrent_heap : heap;
+  concurrent_threads : list thread_state;
+}.
+
+Definition residual_seq (s1 s2 : stmt) : stmt :=
+  match s1 with
+  | SSkip => s2
+  | _ => SSeq s1 s2
+  end.
+
+Inductive thread_step
+    (CT : class_table) :
+    heap -> thread_state -> heap -> thread_state -> Prop :=
+  | TS_AssignInt : forall h rΓ x n old_v,
+      runtime_getVal rΓ x = Some old_v ->
+      thread_step CT h
+        (mkThread rΓ (SVarAss x (EInt n)))
+        h
+        (mkThread (set_vars rΓ (update x (Int n) (vars rΓ))) SSkip)
+
+  | TS_FldWrite : forall h h' rΓ x f y loc_x o a vf val_y,
+      runtime_getVal rΓ x = Some (Iot loc_x) ->
+      runtime_getObj h loc_x = Some o ->
+      getVal (fields_map o) f = Some vf ->
+      sf_assignability_rel CT (rctype (rt_type o)) f a ->
+      runtime_getVal rΓ y = Some val_y ->
+      runtime_vpa_assignability (rqtype (rt_type o)) a = Assignable ->
+      h' = update_field h loc_x f val_y ->
+      thread_step CT h
+        (mkThread rΓ (SFldWrite x f y))
+        h'
+        (mkThread rΓ SSkip)
+
+  | TS_SeqSkip : forall h rΓ s2,
+      thread_step CT h
+        (mkThread rΓ (SSeq SSkip s2))
+        h
+        (mkThread rΓ s2)
+
+  | TS_SeqStep : forall h h' rΓ rΓ' s1 s1' s2,
+      thread_step CT h (mkThread rΓ s1) h' (mkThread rΓ' s1') ->
+      thread_step CT h
+        (mkThread rΓ (SSeq s1 s2))
+        h'
+        (mkThread rΓ' (residual_seq s1' s2)).
+
+Inductive concurrent_step
+    (CT : class_table) :
+    concurrent_config -> concurrent_config -> Prop :=
+  | CS_Thread : forall h h' threads threads' i t t',
+      nth_error threads i = Some t ->
+      thread_step CT h t h' t' ->
+      threads' = update i t' threads ->
+      concurrent_step CT
+        (mkConcurrentConfig h threads)
+        (mkConcurrentConfig h' threads').
+
+Inductive concurrent_steps
+    (CT : class_table) :
+    concurrent_config -> concurrent_config -> Prop :=
+  | CS_Refl : forall cfg,
+      concurrent_steps CT cfg cfg
+  | CS_Step : forall cfg1 cfg2 cfg3,
+      concurrent_step CT cfg1 cfg2 ->
+      concurrent_steps CT cfg2 cfg3 ->
+      concurrent_steps CT cfg1 cfg3.
+
+Definition concurrent_derived_cache_state
+    (CT : class_table) (h : heap) (loc : Loc) (C : class_name)
+    (abs_fields : list var) (cache_f : var)
+    (derived : list value -> nat) : Prop :=
+  exists o,
+    runtime_getObj h loc = Some o /\
+    rctype (rt_type o) = C /\
+    derived_int_cache_protocol CT h loc C abs_fields cache_f derived.
+
+Definition cache_safe_heap_transition
+    (CT : class_table) (h h' : heap) (loc : Loc) (C : class_name)
+    (abs_fields : list var) (cache_f : var)
+    (derived : list value -> nat) : Prop :=
+  h' = h \/
+  exists o abs_vals old_cache_v n,
+    runtime_getObj h loc = Some o /\
+    rctype (rt_type o) = C /\
+    field_reads h loc abs_fields abs_vals /\
+    field_read h loc cache_f old_cache_v /\
+    n = derived abs_vals /\
+    n <> 0 /\
+    h' = update_field h loc cache_f (Int n).
+
+Definition sc_accepts_cache_transition
+    (CT : class_table) (h h' : heap) (loc : Loc) (C : class_name)
+    (abs_fields : list var) (cache_f : var)
+    (derived : list value -> nat) : Prop :=
+  cache_safe_heap_transition CT h h' loc C abs_fields cache_f derived.
+
+Definition sc_rejects_cache_transition
+    (CT : class_table) (h h' : heap) (loc : Loc) (C : class_name)
+    (abs_fields : list var) (cache_f : var)
+    (derived : list value -> nat) : Prop :=
+  not (sc_accepts_cache_transition CT h h' loc C abs_fields cache_f derived).
+
+Lemma sc_accepts_stutter :
+  forall CT h loc C abs_fields cache_f derived,
+    sc_accepts_cache_transition CT h h loc C abs_fields cache_f derived.
+Proof.
+  intros.
+  left.
+  reflexivity.
+Qed.
+
+Lemma sc_accepts_derived_cache_write :
+  forall CT h h' loc C abs_fields cache_f derived abs_vals old_cache_v n o,
+    runtime_getObj h loc = Some o ->
+    rctype (rt_type o) = C ->
+    field_reads h loc abs_fields abs_vals ->
+    field_read h loc cache_f old_cache_v ->
+    n = derived abs_vals ->
+    n <> 0 ->
+    h' = update_field h loc cache_f (Int n) ->
+    sc_accepts_cache_transition CT h h' loc C abs_fields cache_f derived.
+Proof.
+  intros CT h h' loc C abs_fields cache_f derived abs_vals old_cache_v n o
+         Hobj HC Hreads Hcache_read Hderived Hnz Hupdate.
+  right.
+  exists o, abs_vals, old_cache_v, n.
+  repeat split; assumption.
+Qed.
+
+Lemma sc_accepted_transition_preserves_final_reads :
+  forall CT h h' loc C abs_fields cache_f derived abs_vals o,
+    runtime_getObj h loc = Some o ->
+    rctype (rt_type o) = C ->
+    final_fields CT C abs_fields ->
+    cache_field CT C cache_f ->
+    field_reads h loc abs_fields abs_vals ->
+    sc_accepts_cache_transition CT h h' loc C abs_fields cache_f derived ->
+    field_reads h' loc abs_fields abs_vals.
+Proof.
+  intros CT h h' loc C abs_fields cache_f derived abs_vals o
+         Hobj HC Hfinals Hcache Hreads Haccepted.
+  destruct Haccepted as [Heq | Hwrite].
+  - subst h'. exact Hreads.
+  - destruct Hwrite as
+      [o_write [abs_vals_write [old_cache_v [n
+        [Hobj_write [HC_write [Hreads_write
+          [Hcache_read [Hderived [Hnz Hupdate]]]]]]]]]].
+    eapply update_cache_field_preserves_final_field_reads; eauto.
+Qed.
+
+Theorem sc_rejects_final_read_change :
+  forall CT h h' loc C abs_fields cache_f derived abs_vals o,
+    runtime_getObj h loc = Some o ->
+    rctype (rt_type o) = C ->
+    final_fields CT C abs_fields ->
+    cache_field CT C cache_f ->
+    field_reads h loc abs_fields abs_vals ->
+    not (field_reads h' loc abs_fields abs_vals) ->
+    sc_rejects_cache_transition CT h h' loc C abs_fields cache_f derived.
+Proof.
+  intros CT h h' loc C abs_fields cache_f derived abs_vals o
+         Hobj HC Hfinals Hcache Hreads Hchanged Haccepted.
+  apply Hchanged.
+  eapply sc_accepted_transition_preserves_final_reads; eauto.
+Qed.
+
+Lemma cache_safe_heap_transition_preserves_cache_state :
+  forall CT h h' loc C abs_fields cache_f derived,
+    concurrent_derived_cache_state CT h loc C abs_fields cache_f derived ->
+    cache_safe_heap_transition CT h h' loc C abs_fields cache_f derived ->
+    concurrent_derived_cache_state CT h' loc C abs_fields cache_f derived.
+Proof.
+  intros CT h h' loc C abs_fields cache_f derived Hstate Hsafe.
+  destruct Hsafe as [Heq | Hsafe].
+  - subst h'. exact Hstate.
+  - destruct Hsafe as
+      [o [abs_vals [old_cache_v [n
+        [Hobj [HC [Hreads [Hcache_read [Hderived [Hnz Hupdate]]]]]]]]]].
+    destruct Hstate as [o0 [Hobj0 [HC0 Hprotocol]]].
+    assert (o0 = o) by congruence.
+    subst o0.
+    subst h'.
+    exists (set_fields_map o (update cache_f (Int n) (fields_map o))).
+    split.
+    + eapply update_cache_field_preserves_runtime_type; eauto.
+    + split.
+      * simpl. exact HC.
+      * eapply update_known_int_cache_preserves_existing_protocol; eauto.
+Qed.
+
+Theorem concurrent_step_preserves_cache_state :
+  forall CT cfg cfg' loc C abs_fields cache_f derived,
+    concurrent_step CT cfg cfg' ->
+    concurrent_derived_cache_state
+      CT (concurrent_heap cfg) loc C abs_fields cache_f derived ->
+    cache_safe_heap_transition
+      CT (concurrent_heap cfg) (concurrent_heap cfg')
+      loc C abs_fields cache_f derived ->
+    concurrent_derived_cache_state
+      CT (concurrent_heap cfg') loc C abs_fields cache_f derived.
+Proof.
+  intros CT cfg cfg' loc C abs_fields cache_f derived _ Hstate Hsafe.
+  eapply cache_safe_heap_transition_preserves_cache_state; eauto.
+Qed.
+
+Theorem concurrent_steps_preserve_cache_state :
+  forall CT cfg cfg' loc C abs_fields cache_f derived,
+    concurrent_steps CT cfg cfg' ->
+    (forall c1 c2,
+      concurrent_step CT c1 c2 ->
+      cache_safe_heap_transition
+        CT (concurrent_heap c1) (concurrent_heap c2)
+        loc C abs_fields cache_f derived) ->
+    concurrent_derived_cache_state
+      CT (concurrent_heap cfg) loc C abs_fields cache_f derived ->
+    concurrent_derived_cache_state
+      CT (concurrent_heap cfg') loc C abs_fields cache_f derived.
+Proof.
+  intros CT cfg cfg' loc C abs_fields cache_f derived Hsteps Hsafe_all Hstate.
+  induction Hsteps as [cfg0 | cfg1 cfg2 cfg3 Hstep Hsteps_tail IH].
+  - exact Hstate.
+  - apply IH.
+    eapply concurrent_step_preserves_cache_state; eauto.
+Qed.
