ConcurrentPicoExamples.v
@@ -1,0 +1,86 @@
+Require Import Syntax Helpers Bigstep DerivedCache DerivedCacheExamples.
+Require Import ConcurrentPico.
+
+From Stdlib Require Import List.
+Import ListNotations.
+
+Definition simple_sc_initial_heap : heap :=
+  simple_heap (Int 41) (Int 0).
+
+Definition simple_sc_cache_written_heap : heap :=
+  update_field
+    simple_sc_initial_heap simple_loc simple_cache_field
+    (Int (simple_derived [Int 41])).
+
+Definition simple_sc_final_changed_heap : heap :=
+  simple_heap (Int 99) (Int 0).
+
+Lemma simple_sc_accepts_cache_write :
+  sc_accepts_cache_transition
+    simple_CT
+    simple_sc_initial_heap
+    simple_sc_cache_written_heap
+    simple_loc
+    simple_class
+    simple_abs_fields
+    simple_cache_field
+    simple_derived.
+Proof.
+  unfold simple_sc_initial_heap, simple_sc_cache_written_heap.
+  eapply sc_accepts_derived_cache_write
+    with
+      (o := simple_obj (Int 41) (Int 0))
+      (abs_vals := [Int 41])
+      (old_cache_v := Int 0)
+      (n := simple_derived [Int 41]).
+  - reflexivity.
+  - reflexivity.
+  - apply simple_field_reads.
+  - apply simple_cache_read.
+  - reflexivity.
+  - unfold simple_derived. discriminate.
+  - reflexivity.
+Qed.
+
+Lemma simple_final_changed_heap_loses_original_final_read :
+  not
+    (field_reads
+      simple_sc_final_changed_heap
+      simple_loc
+      simple_abs_fields
+      [Int 41]).
+Proof.
+  intro Hreads.
+  unfold simple_sc_final_changed_heap, simple_heap, simple_obj, simple_loc,
+    simple_abs_fields in Hreads.
+  inversion Hreads as [|? ? v vs Hread Htail]; subst.
+  destruct Hread as [o [Hobj Hfield]].
+  simpl in Hobj.
+  inversion Hobj; subst.
+  simpl in Hfield.
+  discriminate.
+Qed.
+
+Lemma simple_sc_rejects_final_field_change :
+  sc_rejects_cache_transition
+    simple_CT
+    simple_sc_initial_heap
+    simple_sc_final_changed_heap
+    simple_loc
+    simple_class
+    simple_abs_fields
+    simple_cache_field
+    simple_derived.
+Proof.
+  unfold simple_sc_initial_heap.
+  eapply sc_rejects_final_read_change
+    with
+      (o := simple_obj (Int 41) (Int 0))
+      (abs_vals := [Int 41]).
+  - reflexivity.
+  - reflexivity.
+  - apply simple_final_fields.
+  - apply simple_cache_field_assignable.
+  - apply simple_field_reads.
+  - apply simple_final_changed_heap_loses_original_final_read.
+Qed.
