DerivedCache.v
@@ -1,0 +1,466 @@
+Require Import Syntax Helpers Typing Bigstep.
+
+From Stdlib Require Import List Lia.
+Import ListNotations.
+
+(* A first, reduced cache layer for the PICO runtime model.
+
+   This file intentionally uses only the reduced core:
+   - object mutability at runtime is still PICO's [Imm_r | Mut_r];
+   - abstract fields are [Final];
+   - cache fields are [Assignable].
+
+   It does not use RO, Lost, RDA, or viewpoint-adapted method scopes. Those
+   remain part of the existing PICO development, but are not needed for the
+   first derived-cache preservation lemmas.
+*)
+
+Definition final_field (CT : class_table) (C : class_name) (f : var) : Prop :=
+  sf_assignability_rel CT C f Final.
+
+Definition cache_field (CT : class_table) (C : class_name) (f : var) : Prop :=
+  sf_assignability_rel CT C f Assignable.
+
+Definition field_read (h : heap) (loc : Loc) (f : var) (v : value) : Prop :=
+  exists o,
+    runtime_getObj h loc = Some o /\
+    getVal (fields_map o) f = Some v.
+
+Definition final_fields (CT : class_table) (C : class_name) (fs : list var) : Prop :=
+  Forall (final_field CT C) fs.
+
+Definition field_reads (h : heap) (loc : Loc) (fs : list var) (vs : list value) : Prop :=
+  Forall2 (field_read h loc) fs vs.
+
+Lemma cache_field_not_final :
+  forall CT C f,
+    cache_field CT C f ->
+    final_field CT C f ->
+    False.
+Proof.
+  intros CT C f Hcache Hfinal.
+  unfold cache_field, final_field in *.
+  pose proof (sf_assignability_deterministic_rel CT C f Assignable Final
+                Hcache Hfinal) as Heq.
+  discriminate Heq.
+Qed.
+
+Lemma cache_field_neq_final_field :
+  forall CT C f_cache f_abs,
+    cache_field CT C f_cache ->
+    final_field CT C f_abs ->
+    f_cache <> f_abs.
+Proof.
+  intros CT C f_cache f_abs Hcache Hfinal Heq.
+  subst f_abs.
+  eapply cache_field_not_final; eauto.
+Qed.
+
+Lemma update_cache_field_preserves_final_field_read :
+  forall CT h h' loc C f_cache f_abs new_v old_v o,
+    runtime_getObj h loc = Some o ->
+    rctype (rt_type o) = C ->
+    cache_field CT C f_cache ->
+    final_field CT C f_abs ->
+    getVal (fields_map o) f_abs = Some old_v ->
+    h' = update_field h loc f_cache new_v ->
+    field_read h' loc f_abs old_v.
+Proof.
+  intros CT h h' loc C f_cache f_abs new_v old_v o
+         Hobj HC Hcache Hfinal Hread Hupdate.
+  subst h'.
+  unfold field_read.
+  unfold update_field.
+  rewrite Hobj.
+  exists (set_fields_map o (update f_cache new_v (fields_map o))).
+  split.
+  - apply runtime_getObj_update_same.
+    eapply runtime_getObj_dom; eauto.
+  - simpl.
+    rewrite (field_update_preserves_other_fields
+               (fields_map o) f_cache new_v f_abs).
+    + eapply cache_field_neq_final_field; eauto.
+    + exact Hread.
+Qed.
+
+Lemma update_cache_field_preserves_runtime_type :
+  forall h loc f_cache new_v o,
+    runtime_getObj h loc = Some o ->
+    runtime_getObj (update_field h loc f_cache new_v) loc =
+      Some (set_fields_map o (update f_cache new_v (fields_map o))).
+Proof.
+  intros h loc f_cache new_v o Hobj.
+  unfold update_field.
+  rewrite Hobj.
+  apply runtime_getObj_update_same.
+  eapply runtime_getObj_dom; eauto.
+Qed.
+
+Lemma update_cache_field_preserves_final_field_reads :
+  forall CT h h' loc C f_cache new_v fs vs o,
+    runtime_getObj h loc = Some o ->
+    rctype (rt_type o) = C ->
+    cache_field CT C f_cache ->
+    final_fields CT C fs ->
+    field_reads h loc fs vs ->
+    h' = update_field h loc f_cache new_v ->
+    field_reads h' loc fs vs.
+Proof.
+  intros CT h h' loc C f_cache new_v fs vs o
+         Hobj HC Hcache Hfinals Hreads Hupdate.
+  unfold final_fields in Hfinals.
+  unfold field_reads in *.
+  generalize dependent vs.
+  induction Hfinals as [|f_abs fs Hfinal Hfinals_tail IH]; intros vs Hreads.
+  - inversion Hreads; constructor.
+  - inversion Hreads as [|? ? old_v vs_tail Hread Hreads_tail0]; subst.
+    constructor.
+    + destruct Hread as [o_read [Hobj_read Hfield_read]].
+      assert (o_read = o) by congruence.
+      subst o_read.
+      eapply update_cache_field_preserves_final_field_read; eauto.
+    + eapply IH; eauto.
+Qed.
+
+Definition cache_value_unknown (v : value) : Prop :=
+  v = Int 0.
+
+Definition cache_value_known (derived : list value -> nat) (abs_vals : list value)
+  (v : value) : Prop :=
+  exists n,
+    v = Int n /\
+    n = derived abs_vals /\
+    n <> 0.
+
+Definition derived_int_cache_value
+  (derived : list value -> nat) (abs_vals : list value) (v : value) : Prop :=
+  cache_value_unknown v \/ cache_value_known derived abs_vals v.
+
+Definition derived_int_cache_protocol
+  (CT : class_table) (h : heap) (loc : Loc) (C : class_name)
+  (abs_fields : list var) (cache_f : var) (derived : list value -> nat) : Prop :=
+  exists abs_vals cache_v,
+    final_fields CT C abs_fields /\
+    cache_field CT C cache_f /\
+    field_reads h loc abs_fields abs_vals /\
+    field_read h loc cache_f cache_v /\
+    derived_int_cache_value derived abs_vals cache_v.
+
+Lemma cache_value_known_intro :
+  forall derived abs_vals n,
+    n = derived abs_vals ->
+    n <> 0 ->
+    cache_value_known derived abs_vals (Int n).
+Proof.
+  intros derived abs_vals n Hderived Hnz.
+  exists n.
+  repeat split; auto.
+Qed.
+
+Lemma derived_int_cache_value_known_intro :
+  forall derived abs_vals n,
+    n = derived abs_vals ->
+    n <> 0 ->
+    derived_int_cache_value derived abs_vals (Int n).
+Proof.
+  intros derived abs_vals n Hderived Hnz.
+  right.
+  apply cache_value_known_intro; assumption.
+Qed.
+
+Lemma update_known_int_cache_preserves_protocol :
+  forall CT h h' loc C abs_fields cache_f derived abs_vals old_cache_v n o,
+    runtime_getObj h loc = Some o ->
+    rctype (rt_type o) = C ->
+    final_fields CT C abs_fields ->
+    cache_field CT C cache_f ->
+    field_reads h loc abs_fields abs_vals ->
+    field_read h loc cache_f old_cache_v ->
+    n = derived abs_vals ->
+    n <> 0 ->
+    h' = update_field h loc cache_f (Int n) ->
+    derived_int_cache_protocol CT h' loc C abs_fields cache_f derived.
+Proof.
+  intros CT h h' loc C abs_fields cache_f derived abs_vals old_cache_v n o
+         Hobj HC Hfinals Hcache Hreads Hcache_read Hderived Hnz Hupdate.
+  exists abs_vals, (Int n).
+  repeat split.
+  - exact Hfinals.
+  - exact Hcache.
+  - eapply update_cache_field_preserves_final_field_reads; eauto.
+  - subst h'.
+    unfold field_read.
+    exists (set_fields_map o (update cache_f (Int n) (fields_map o))).
+    unfold update_field.
+    rewrite Hobj.
+    split.
+    + apply runtime_getObj_update_same.
+      eapply runtime_getObj_dom; eauto.
+    + simpl.
+      unfold getVal.
+      apply update_same.
+      destruct Hcache_read as [o_read [Hobj_read Hfield_read]].
+      assert (o_read = o) by congruence.
+      subst o_read.
+      eapply getVal_dom; eauto.
+  - apply derived_int_cache_value_known_intro; assumption.
+Qed.
+
+Lemma update_known_int_cache_preserves_existing_protocol :
+  forall CT h h' loc C abs_fields cache_f derived abs_vals old_cache_v n o,
+    derived_int_cache_protocol CT h loc C abs_fields cache_f derived ->
+    runtime_getObj h loc = Some o ->
+    rctype (rt_type o) = C ->
+    field_reads h loc abs_fields abs_vals ->
+    field_read h loc cache_f old_cache_v ->
+    n = derived abs_vals ->
+    n <> 0 ->
+    h' = update_field h loc cache_f (Int n) ->
+    derived_int_cache_protocol CT h' loc C abs_fields cache_f derived.
+Proof.
+  intros CT h h' loc C abs_fields cache_f derived abs_vals old_cache_v n o
+         Hprotocol Hobj HC Hreads Hcache_read Hderived Hnz Hupdate.
+  destruct Hprotocol as [abs_vals0 [cache_v
+    [Hfinals [Hcache [_ [_ _]]]]]].
+  eapply update_known_int_cache_preserves_protocol; eauto.
+Qed.
+
+Lemma eval_cache_field_write_establishes_protocol :
+  forall CT rΓ h h' x y loc C abs_fields cache_f derived
+         abs_vals old_cache_v n o,
+    eval_stmt
+      OK
+      (reachable_locations_from_initial_env CT h rΓ)
+      CT rΓ h
+      (SFldWrite x cache_f y)
+      OK
+      (reachable_locations_from_initial_env CT h rΓ)
+      rΓ h' ->
+    runtime_getVal rΓ x = Some (Iot loc) ->
+    runtime_getVal rΓ y = Some (Int n) ->
+    runtime_getObj h loc = Some o ->
+    rctype (rt_type o) = C ->
+    final_fields CT C abs_fields ->
+    cache_field CT C cache_f ->
+    field_reads h loc abs_fields abs_vals ->
+    field_read h loc cache_f old_cache_v ->
+    n = derived abs_vals ->
+    n <> 0 ->
+    derived_int_cache_protocol CT h' loc C abs_fields cache_f derived.
+Proof.
+  intros CT rΓ h h' x y loc C abs_fields cache_f derived
+         abs_vals old_cache_v n o
+         Heval Hx Hy Hobj HC Hfinals Hcache Hreads Hcache_read Hderived Hnz.
+  pose (n_cache := n).
+  assert (Hy_cache : runtime_getVal rΓ y = Some (Int n_cache))
+    by (unfold n_cache; exact Hy).
+  inversion Heval; subst; try discriminate.
+  assert (loc_x = loc) by congruence.
+  assert (val_y = Int n_cache) by congruence.
+  subst loc_x val_y.
+  eapply update_known_int_cache_preserves_protocol
+    with (n := n_cache) (old_cache_v := old_cache_v); eauto.
+Qed.
+
+Lemma eval_cache_field_write_preserves_final_reads :
+  forall CT rΓ h h' x y loc C abs_fields cache_f abs_vals o,
+    eval_stmt
+      OK
+      (reachable_locations_from_initial_env CT h rΓ)
+      CT rΓ h
+      (SFldWrite x cache_f y)
+      OK
+      (reachable_locations_from_initial_env CT h rΓ)
+      rΓ h' ->
+    runtime_getVal rΓ x = Some (Iot loc) ->
+    runtime_getObj h loc = Some o ->
+    rctype (rt_type o) = C ->
+    final_fields CT C abs_fields ->
+    cache_field CT C cache_f ->
+    field_reads h loc abs_fields abs_vals ->
+    field_reads h' loc abs_fields abs_vals.
+Proof.
+  intros CT rΓ h h' x y loc C abs_fields cache_f abs_vals o
+         Heval Hx Hobj HC Hfinals Hcache Hreads.
+  inversion Heval; subst; try discriminate.
+  assert (loc_x = loc) by congruence.
+  subst loc_x.
+  eapply update_cache_field_preserves_final_field_reads; eauto.
+Qed.
+
+Lemma eval_int_compute_and_cache_write_sound :
+  forall CT rΓ rΓ_mid h h' receiver tmp loc C abs_fields cache_f derived
+         abs_vals old_cache_v n o,
+    eval_stmt
+      OK
+      (reachable_locations_from_initial_env CT h rΓ)
+      CT rΓ h
+      (SVarAss tmp (EInt n))
+      OK
+      (reachable_locations_from_initial_env CT h rΓ)
+      rΓ_mid h ->
+    eval_stmt
+      OK
+      (reachable_locations_from_initial_env CT h rΓ_mid)
+      CT rΓ_mid h
+      (SFldWrite receiver cache_f tmp)
+      OK
+      (reachable_locations_from_initial_env CT h rΓ_mid)
+      rΓ_mid h' ->
+    runtime_getVal rΓ_mid receiver = Some (Iot loc) ->
+    runtime_getVal rΓ_mid tmp = Some (Int n) ->
+    runtime_getObj h loc = Some o ->
+    rctype (rt_type o) = C ->
+    final_fields CT C abs_fields ->
+    cache_field CT C cache_f ->
+    field_reads h loc abs_fields abs_vals ->
+    field_read h loc cache_f old_cache_v ->
+    n = derived abs_vals ->
+    n <> 0 ->
+    field_reads h' loc abs_fields abs_vals /\
+    derived_int_cache_protocol CT h' loc C abs_fields cache_f derived.
+Proof.
+  intros CT rΓ rΓ_mid h h' receiver tmp loc C abs_fields cache_f derived
+         abs_vals old_cache_v n o
+         _ Hwrite Hreceiver_mid Htmp_mid Hobj HC Hfinals Hcache Hreads
+         Hcache_read Hderived Hnz.
+  split.
+  - eapply eval_cache_field_write_preserves_final_reads; eauto.
+  - eapply eval_cache_field_write_establishes_protocol; eauto.
+Qed.
+
+Theorem derived_cache_update_immutability :
+  forall CT sΓ mt rΓ rΓ_mid h h' receiver tmp loc C abs_fields cache_f
+         abs_vals n o,
+    wf_r_config CT sΓ rΓ h ->
+    stmt_typing CT sΓ mt (SVarAss tmp (EInt n)) sΓ ->
+    stmt_typing CT sΓ mt (SFldWrite receiver cache_f tmp) sΓ ->
+    eval_stmt
+      OK
+      (reachable_locations_from_initial_env CT h rΓ)
+      CT rΓ h
+      (SVarAss tmp (EInt n))
+      OK
+      (reachable_locations_from_initial_env CT h rΓ)
+      rΓ_mid h ->
+    eval_stmt
+      OK
+      (reachable_locations_from_initial_env CT h rΓ_mid)
+      CT rΓ_mid h
+      (SFldWrite receiver cache_f tmp)
+      OK
+      (reachable_locations_from_initial_env CT h rΓ_mid)
+      rΓ_mid h' ->
+    runtime_getVal rΓ_mid receiver = Some (Iot loc) ->
+    runtime_getObj h loc = Some o ->
+    rctype (rt_type o) = C ->
+    final_fields CT C abs_fields ->
+    cache_field CT C cache_f ->
+    field_reads h loc abs_fields abs_vals ->
+    field_reads h' loc abs_fields abs_vals.
+Proof.
+  intros CT sΓ mt rΓ rΓ_mid h h' receiver tmp loc C abs_fields cache_f
+         abs_vals n o
+         _ _ _ _ Hwrite Hreceiver_mid Hobj HC Hfinals Hcache Hreads.
+  eapply eval_cache_field_write_preserves_final_reads; eauto.
+Qed.
+
+Theorem derived_cache_update_sound :
+  forall CT sΓ mt rΓ rΓ_mid h h' receiver tmp loc C abs_fields cache_f
+         derived abs_vals old_cache_v n o,
+    wf_r_config CT sΓ rΓ h ->
+    stmt_typing CT sΓ mt (SVarAss tmp (EInt n)) sΓ ->
+    stmt_typing CT sΓ mt (SFldWrite receiver cache_f tmp) sΓ ->
+    eval_stmt
+      OK
+      (reachable_locations_from_initial_env CT h rΓ)
+      CT rΓ h
+      (SVarAss tmp (EInt n))
+      OK
+      (reachable_locations_from_initial_env CT h rΓ)
+      rΓ_mid h ->
+    eval_stmt
+      OK
+      (reachable_locations_from_initial_env CT h rΓ_mid)
+      CT rΓ_mid h
+      (SFldWrite receiver cache_f tmp)
+      OK
+      (reachable_locations_from_initial_env CT h rΓ_mid)
+      rΓ_mid h' ->
+    runtime_getVal rΓ_mid receiver = Some (Iot loc) ->
+    runtime_getVal rΓ_mid tmp = Some (Int n) ->
+    runtime_getObj h loc = Some o ->
+    rctype (rt_type o) = C ->
+    final_fields CT C abs_fields ->
+    cache_field CT C cache_f ->
+    field_reads h loc abs_fields abs_vals ->
+    field_read h loc cache_f old_cache_v ->
+    n = derived abs_vals ->
+    n <> 0 ->
+    field_reads h' loc abs_fields abs_vals /\
+    derived_int_cache_protocol CT h' loc C abs_fields cache_f derived.
+Proof.
+  intros CT sΓ mt rΓ rΓ_mid h h' receiver tmp loc C abs_fields cache_f
+         derived abs_vals old_cache_v n o
+         _ _ _ Hcompute Hwrite Hreceiver_mid Htmp_mid Hobj HC Hfinals Hcache
+         Hreads Hcache_read Hderived Hnz.
+  eapply eval_int_compute_and_cache_write_sound; eauto.
+Qed.
+
+(* PICO's current big-step semantics is sequential. It has no thread pool,
+   interleaving semantics, data-race relation, or memory model. The theorem
+   below is therefore a sequential semantic soundness theorem for the concrete
+   cache-update sequence shape.
+
+   The explicit reachability-stability premise is needed because [SBS_Seq]
+   threads the initial reachability set through the second statement, while
+   primitive statement rules recompute reachability from their own input
+   runtime environment. Assigning an integer temporary does not add reachable
+   locations, so examples can discharge this premise directly. *)
+Theorem derived_cache_update_sequence_sound :
+  forall CT sΓ mt rΓ rΓ_mid h h' receiver tmp loc C abs_fields cache_f
+         derived abs_vals old_cache_v n o,
+    wf_r_config CT sΓ rΓ h ->
+    stmt_typing CT sΓ mt (SVarAss tmp (EInt n)) sΓ ->
+    stmt_typing CT sΓ mt (SFldWrite receiver cache_f tmp) sΓ ->
+    rΓ_mid = set_vars rΓ (update tmp (Int n) (vars rΓ)) ->
+    reachable_locations_from_initial_env CT h rΓ_mid =
+      reachable_locations_from_initial_env CT h rΓ ->
+    eval_stmt
+      OK
+      (reachable_locations_from_initial_env CT h rΓ)
+      CT rΓ h
+      (SSeq (SVarAss tmp (EInt n)) (SFldWrite receiver cache_f tmp))
+      OK
+      (reachable_locations_from_initial_env CT h rΓ)
+      rΓ_mid h' ->
+    runtime_getVal rΓ_mid receiver = Some (Iot loc) ->
+    runtime_getVal rΓ_mid tmp = Some (Int n) ->
+    runtime_getObj h loc = Some o ->
+    rctype (rt_type o) = C ->
+    final_fields CT C abs_fields ->
+    cache_field CT C cache_f ->
+    field_reads h loc abs_fields abs_vals ->
+    field_read h loc cache_f old_cache_v ->
+    n = derived abs_vals ->
+    n <> 0 ->
+    field_reads h' loc abs_fields abs_vals /\
+    derived_int_cache_protocol CT h' loc C abs_fields cache_f derived.
+Proof.
+  intros CT sΓ mt rΓ rΓ_mid h h' receiver tmp loc C abs_fields cache_f
+         derived abs_vals old_cache_v n o
+         Hwf Htype_compute Htype_write Hmid Hreach_stable Hseq
+         Hreceiver_mid Htmp_mid Hobj HC Hfinals Hcache Hreads Hcache_read
+         Hderived Hnz.
+  subst rΓ_mid.
+  inversion Hseq; subst; try discriminate.
+  inversion Heval1; subst; try discriminate.
+  inversion Heval; subst; try discriminate.
+  rewrite <- Hreach_stable in Heval2.
+  eapply derived_cache_update_sound
+    with
+      (sΓ := sΓ)
+      (mt := mt)
+      (old_cache_v := old_cache_v)
+      (o := o); eauto.
+Qed.
