DerivedCacheExamples.v
@@ -1,0 +1,547 @@
+Require Import Syntax Helpers Typing Bigstep DerivedCache ViewpointAdaptation Subtyping.
+
+From Stdlib Require Import List Lia.
+From Stdlib Require Import Logic.FunctionalExtensionality.
+From Stdlib Require Import Logic.PropExtensionality.
+Import ListNotations.
+
+Definition simple_value_field : var := 0.
+Definition simple_cache_field : var := 1.
+Definition simple_root_class : class_name := 0.
+Definition simple_class : class_name := 1.
+
+Definition simple_value_field_def : field_def :=
+  {|
+    ftype :=
+      {|
+        assignability := Final;
+        mutability := Imm_f;
+        f_base_type := simple_class
+      |};
+    fname := simple_value_field
+  |}.
+
+Definition simple_cache_field_def : field_def :=
+  {|
+    ftype :=
+      {|
+        assignability := Assignable;
+        mutability := Imm_f;
+        f_base_type := int_class_name
+      |};
+    fname := simple_cache_field
+  |}.
+
+Definition simple_constructor : constructor_def :=
+  {|
+    csignature :=
+      {|
+        cqualifier := Imm_c;
+        cparams := []
+      |}
+  |}.
+
+Definition simple_root_class_def : class_def :=
+  {|
+    signature :=
+      {|
+        class_qualifier := Imm_c;
+        cname := simple_root_class;
+        super := None
+      |};
+    body :=
+      {|
+        fields := [];
+        constructor := simple_constructor;
+        methods := []
+      |}
+  |}.
+
+Definition simple_class_def : class_def :=
+  {|
+    signature :=
+      {|
+        class_qualifier := Imm_c;
+        cname := simple_class;
+        super := Some simple_root_class
+      |};
+    body :=
+      {|
+        fields := [simple_value_field_def; simple_cache_field_def];
+        constructor := simple_constructor;
+        methods := []
+      |}
+  |}.
+
+Definition simple_CT : class_table := [simple_root_class_def; simple_class_def].
+
+Definition simple_obj (abstract_v cache_v : value) : Obj :=
+  mkObj
+    (mkruntime_type Imm_r simple_class)
+    [abstract_v; cache_v].
+
+Definition simple_heap (abstract_v cache_v : value) : heap :=
+  [simple_obj abstract_v cache_v].
+
+Definition simple_loc : Loc := 0.
+
+Definition simple_abs_fields : list var := [simple_value_field].
+
+Definition simple_derived (vs : list value) : nat :=
+  match vs with
+  | [Int n] => S n
+  | _ => 1
+  end.
+
+Definition simple_cache_tmp_var : var := 1.
+
+Definition simple_cache_env (derived_v : value) : r_env :=
+  mkr_env [Iot simple_loc; derived_v].
+
+Definition simple_cache_write_stmt : stmt :=
+  SFldWrite 0 simple_cache_field simple_cache_tmp_var.
+
+Definition simple_cache_compute_stmt : stmt :=
+  SVarAss simple_cache_tmp_var (EInt (simple_derived [Int 41])).
+
+Definition simple_cache_compute_and_write_stmt : stmt :=
+  SSeq simple_cache_compute_stmt simple_cache_write_stmt.
+
+Definition simple_cache_senv : s_env :=
+  [Build_qualified_type Imm simple_class; int_type].
+
+Lemma simple_value_field_final :
+  final_field simple_CT simple_class simple_value_field.
+Proof.
+  unfold final_field, sf_assignability_rel, simple_CT, simple_class,
+    simple_value_field.
+  exists simple_value_field_def.
+  split.
+  - apply FL_Found with
+      (fields := [] ++ [simple_value_field_def; simple_cache_field_def]).
+    + eapply CF_Inherit.
+      * reflexivity.
+      * reflexivity.
+      * apply CF_Object with (def := simple_root_class_def); reflexivity.
+      * reflexivity.
+    + reflexivity.
+  - reflexivity.
+Qed.
+
+Lemma simple_cache_field_assignable :
+  cache_field simple_CT simple_class simple_cache_field.
+Proof.
+  unfold cache_field, sf_assignability_rel, simple_CT, simple_class,
+    simple_cache_field.
+  exists simple_cache_field_def.
+  split.
+  - apply FL_Found with
+      (fields := [] ++ [simple_value_field_def; simple_cache_field_def]).
+    + eapply CF_Inherit.
+      * reflexivity.
+      * reflexivity.
+      * apply CF_Object with (def := simple_root_class_def); reflexivity.
+      * reflexivity.
+    + reflexivity.
+  - reflexivity.
+Qed.
+
+Lemma simple_final_fields :
+  final_fields simple_CT simple_class simple_abs_fields.
+Proof.
+  unfold final_fields, simple_abs_fields.
+  constructor.
+  - apply simple_value_field_final.
+  - constructor.
+Qed.
+
+Lemma simple_field_reads :
+  forall abstract_v cache_v,
+    field_reads (simple_heap abstract_v cache_v) simple_loc simple_abs_fields
+      [abstract_v].
+Proof.
+  intros abstract_v cache_v.
+  unfold field_reads, simple_heap, simple_obj, simple_loc, simple_abs_fields.
+  constructor.
+  - unfold field_read.
+    exists (mkObj (mkruntime_type Imm_r simple_class) [abstract_v; cache_v]).
+    split; reflexivity.
+  - constructor.
+Qed.
+
+Lemma simple_cache_read :
+  forall abstract_v cache_v,
+    field_read (simple_heap abstract_v cache_v) simple_loc simple_cache_field
+      cache_v.
+Proof.
+  intros abstract_v cache_v.
+  unfold field_read, simple_heap, simple_obj, simple_loc, simple_cache_field.
+  exists (mkObj (mkruntime_type Imm_r simple_class) [abstract_v; cache_v]).
+  split; reflexivity.
+Qed.
+
+Lemma simple_object_lookup :
+  forall abstract_v cache_v,
+    runtime_getObj (simple_heap abstract_v cache_v) simple_loc =
+      Some (simple_obj abstract_v cache_v).
+Proof.
+  reflexivity.
+Qed.
+
+Lemma simple_cache_senv_wf :
+  wf_senv simple_CT simple_cache_senv.
+Proof.
+  unfold wf_senv, simple_cache_senv, wf_stypeuse, simple_CT,
+    simple_class, int_type, int_class_name, bound, find_class, gget,
+    vpa_mutability_bound.
+  simpl.
+  repeat split; try lia; repeat constructor; discriminate.
+Qed.
+
+Lemma simple_int_literal_typed :
+  expr_has_type simple_CT simple_cache_senv SafeRO
+    (EInt (simple_derived [Int 41]))
+    int_type.
+Proof.
+  apply ET_Int.
+  - apply simple_cache_senv_wf.
+  - unfold int_class_name, simple_CT. simpl. lia.
+Qed.
+
+Lemma simple_assign_literal_typed :
+  stmt_typing simple_CT simple_cache_senv SafeRO
+    simple_cache_compute_stmt
+    simple_cache_senv.
+Proof.
+  unfold simple_cache_compute_stmt.
+  eapply ST_VarAss with
+    (Te := int_type)
+    (Tthis := Build_qualified_type Imm simple_class)
+    (Tx := int_type).
+  - apply simple_cache_senv_wf.
+  - apply simple_int_literal_typed.
+  - reflexivity.
+  - unfold simple_cache_tmp_var. discriminate.
+  - reflexivity.
+  - apply qtype_refl.
+    + unfold int_type, int_class_name, simple_CT. simpl. lia.
+    + unfold int_type. simpl. discriminate.
+Qed.
+
+Lemma simple_int_literal_eval :
+  eval_expr
+    OK
+    (reachable_locations_from_initial_env
+       simple_CT
+       (simple_heap (Int 41) (Int 0))
+       (simple_cache_env (Int 0)))
+    simple_CT
+    (simple_cache_env (Int 0))
+    (simple_heap (Int 41) (Int 0))
+    (EInt (simple_derived [Int 41]))
+    (Int (simple_derived [Int 41]))
+    OK
+    (reachable_locations_from_initial_env
+       simple_CT
+       (simple_heap (Int 41) (Int 0))
+       (simple_cache_env (Int 0)))
+    (simple_cache_env (Int 0))
+    (simple_heap (Int 41) (Int 0)).
+Proof.
+  apply EBS_Int.
+Qed.
+
+Lemma simple_assign_literal_eval :
+  eval_stmt
+    OK
+    (reachable_locations_from_initial_env
+       simple_CT
+       (simple_heap (Int 41) (Int 0))
+       (simple_cache_env (Int 0)))
+    simple_CT
+    (simple_cache_env (Int 0))
+    (simple_heap (Int 41) (Int 0))
+    simple_cache_compute_stmt
+    OK
+    (reachable_locations_from_initial_env
+       simple_CT
+       (simple_heap (Int 41) (Int 0))
+       (simple_cache_env (Int 0)))
+    (simple_cache_env (Int (simple_derived [Int 41])))
+    (simple_heap (Int 41) (Int 0)).
+Proof.
+  unfold simple_cache_compute_stmt, simple_cache_env, simple_cache_tmp_var,
+    simple_derived.
+  simpl.
+  change {| vars := [Iot simple_loc; Int 42] |} with
+    (set_vars {| vars := [Iot simple_loc; Int 0] |}
+      (update 1 (Int 42) [Iot simple_loc; Int 0])).
+  eapply SBS_Assign with (v1 := Int 0).
+  - reflexivity.
+  - apply EBS_Int.
+Qed.
+
+Lemma simple_cache_write_typed :
+  stmt_typing simple_CT simple_cache_senv SafeRO
+    simple_cache_write_stmt
+    simple_cache_senv.
+Proof.
+  unfold simple_cache_write_stmt.
+  eapply ST_FldWrite_safe_ro with
+    (Tx := Build_qualified_type Imm simple_class)
+    (Ty := int_type)
+    (Tthis := Build_qualified_type Imm simple_class)
+    (fieldT := simple_cache_field_def)
+    (a := Assignable).
+  - apply simple_cache_senv_wf.
+  - reflexivity.
+  - reflexivity.
+  - reflexivity.
+  - unfold sf_def_rel, simple_CT, simple_class, simple_cache_field.
+    apply FL_Found with
+      (fields := [] ++ [simple_value_field_def; simple_cache_field_def]).
+    + eapply CF_Inherit.
+      * reflexivity.
+      * reflexivity.
+      * apply CF_Object with (def := simple_root_class_def); reflexivity.
+      * reflexivity.
+    + reflexivity.
+  - apply simple_cache_field_assignable.
+  - apply qtype_refl.
+    + change (0 < 2). lia.
+    + unfold int_type. simpl. discriminate.
+  - reflexivity.
+Qed.
+
+Lemma simple_cache_compute_and_write_typed :
+  stmt_typing simple_CT simple_cache_senv SafeRO
+    simple_cache_compute_and_write_stmt
+    simple_cache_senv.
+Proof.
+  unfold simple_cache_compute_and_write_stmt.
+  eapply ST_Seq with (sΓ' := simple_cache_senv).
+  - apply simple_cache_senv_wf.
+  - apply simple_assign_literal_typed.
+  - apply simple_cache_write_typed.
+Qed.
+
+Lemma simple_update_known_cache_protocol :
+    derived_int_cache_protocol
+      simple_CT
+      (update_field (simple_heap (Int 41) (Int 0)) simple_loc
+         simple_cache_field (Int (simple_derived [Int 41])))
+      simple_loc
+      simple_class
+      simple_abs_fields
+      simple_cache_field
+      simple_derived.
+Proof.
+  eapply update_known_int_cache_preserves_protocol
+    with
+      (h := simple_heap (Int 41) (Int 0))
+      (o := simple_obj (Int 41) (Int 0))
+      (abs_vals := [Int 41])
+      (old_cache_v := Int 0).
+  - apply simple_object_lookup.
+  - reflexivity.
+  - apply simple_final_fields.
+  - apply simple_cache_field_assignable.
+  - apply simple_field_reads.
+  - apply simple_cache_read.
+  - unfold simple_derived. reflexivity.
+  - unfold simple_derived. lia.
+  - reflexivity.
+Qed.
+
+Lemma simple_cache_write_eval :
+  eval_stmt
+    OK
+    (reachable_locations_from_initial_env
+       simple_CT
+       (simple_heap (Int 41) (Int 0))
+       (simple_cache_env (Int (simple_derived [Int 41]))))
+    simple_CT
+    (simple_cache_env (Int (simple_derived [Int 41])))
+    (simple_heap (Int 41) (Int 0))
+    simple_cache_write_stmt
+    OK
+    (reachable_locations_from_initial_env
+       simple_CT
+       (simple_heap (Int 41) (Int 0))
+       (simple_cache_env (Int (simple_derived [Int 41]))))
+    (simple_cache_env (Int (simple_derived [Int 41])))
+    (update_field (simple_heap (Int 41) (Int 0)) simple_loc
+       simple_cache_field (Int (simple_derived [Int 41]))).
+Proof.
+  unfold simple_cache_write_stmt.
+  eapply SBS_FldWrite
+    with
+      (loc_x := simple_loc)
+      (o := simple_obj (Int 41) (Int 0))
+      (a := Assignable)
+      (vf := Int 0)
+      (val_y := Int (simple_derived [Int 41])).
+  - unfold simple_cache_env, simple_loc. reflexivity.
+  - apply simple_object_lookup.
+  - unfold simple_obj, simple_cache_field. reflexivity.
+  - apply simple_cache_field_assignable.
+  - unfold simple_cache_env, simple_cache_tmp_var. reflexivity.
+  - reflexivity.
+  - reflexivity.
+Qed.
+
+Lemma simple_cache_write_eval_protocol :
+  exists h',
+    eval_stmt
+      OK
+      (reachable_locations_from_initial_env
+         simple_CT
+         (simple_heap (Int 41) (Int 0))
+         (simple_cache_env (Int (simple_derived [Int 41]))))
+      simple_CT
+      (simple_cache_env (Int (simple_derived [Int 41])))
+      (simple_heap (Int 41) (Int 0))
+      simple_cache_write_stmt
+      OK
+      (reachable_locations_from_initial_env
+         simple_CT
+         (simple_heap (Int 41) (Int 0))
+         (simple_cache_env (Int (simple_derived [Int 41]))))
+      (simple_cache_env (Int (simple_derived [Int 41])))
+      h' /\
+    derived_int_cache_protocol
+      simple_CT
+      h'
+      simple_loc
+      simple_class
+      simple_abs_fields
+      simple_cache_field
+      simple_derived.
+Proof.
+  exists (update_field (simple_heap (Int 41) (Int 0)) simple_loc
+            simple_cache_field (Int (simple_derived [Int 41]))).
+  split.
+  - apply simple_cache_write_eval.
+  - eapply eval_cache_field_write_establishes_protocol
+      with
+        (rΓ := simple_cache_env (Int (simple_derived [Int 41])))
+        (x := 0)
+        (y := simple_cache_tmp_var)
+        (o := simple_obj (Int 41) (Int 0))
+        (abs_vals := [Int 41])
+        (old_cache_v := Int 0)
+        (n := simple_derived [Int 41]).
+    + apply simple_cache_write_eval.
+    + unfold simple_cache_env, simple_loc. reflexivity.
+    + unfold simple_cache_env, simple_cache_tmp_var. reflexivity.
+    + apply simple_object_lookup.
+    + reflexivity.
+    + apply simple_final_fields.
+    + apply simple_cache_field_assignable.
+    + apply simple_field_reads.
+    + apply simple_cache_read.
+    + unfold simple_derived. reflexivity.
+    + unfold simple_derived. lia.
+Qed.
+
+Lemma simple_cache_reachable_ignores_tmp_int :
+  forall n1 n2,
+    reachable_locations_from_initial_env
+      simple_CT
+      (simple_heap (Int 41) (Int 0))
+      (simple_cache_env (Int n1)) =
+    reachable_locations_from_initial_env
+      simple_CT
+      (simple_heap (Int 41) (Int 0))
+      (simple_cache_env (Int n2)).
+Proof.
+  intros n1 n2.
+  apply functional_extensionality.
+  intro l_target.
+  apply propositional_extensionality.
+  unfold reachable_locations_from_initial_env, simple_cache_env.
+  split; intros [x [l_root [Hroot Hreach]]].
+  - destruct x as [|x].
+    + simpl in Hroot.
+      injection Hroot as ?; subst.
+      exists 0, simple_loc. split; [reflexivity | exact Hreach].
+    + destruct x as [|x].
+      * unfold runtime_getVal, simple_cache_env in Hroot.
+        simpl in Hroot. discriminate Hroot.
+      * unfold runtime_getVal, simple_cache_env in Hroot.
+        destruct x; simpl in Hroot; discriminate Hroot.
+  - destruct x as [|x].
+    + simpl in Hroot.
+      injection Hroot as ?; subst.
+      exists 0, simple_loc. split; [reflexivity | exact Hreach].
+    + destruct x as [|x].
+      * unfold runtime_getVal, simple_cache_env in Hroot.
+        simpl in Hroot. discriminate Hroot.
+      * unfold runtime_getVal, simple_cache_env in Hroot.
+        destruct x; simpl in Hroot; discriminate Hroot.
+Qed.
+
+Lemma simple_cache_compute_and_write_eval :
+  eval_stmt
+    OK
+    (reachable_locations_from_initial_env
+       simple_CT
+       (simple_heap (Int 41) (Int 0))
+       (simple_cache_env (Int 0)))
+    simple_CT
+    (simple_cache_env (Int 0))
+    (simple_heap (Int 41) (Int 0))
+    simple_cache_compute_and_write_stmt
+    OK
+    (reachable_locations_from_initial_env
+       simple_CT
+       (simple_heap (Int 41) (Int 0))
+       (simple_cache_env (Int 0)))
+    (simple_cache_env (Int (simple_derived [Int 41])))
+    (update_field (simple_heap (Int 41) (Int 0)) simple_loc
+       simple_cache_field (Int (simple_derived [Int 41]))).
+Proof.
+  unfold simple_cache_compute_and_write_stmt.
+  eapply SBS_Seq with
+    (rΓ' := simple_cache_env (Int (simple_derived [Int 41])))
+    (h' := simple_heap (Int 41) (Int 0)).
+  - apply simple_assign_literal_eval.
+  - rewrite (simple_cache_reachable_ignores_tmp_int
+               0 (simple_derived [Int 41])).
+    apply simple_cache_write_eval.
+Qed.
+
+Lemma simple_cache_compute_and_write_eval_protocol :
+  exists h',
+    eval_stmt
+      OK
+      (reachable_locations_from_initial_env
+         simple_CT
+         (simple_heap (Int 41) (Int 0))
+         (simple_cache_env (Int 0)))
+      simple_CT
+      (simple_cache_env (Int 0))
+      (simple_heap (Int 41) (Int 0))
+      simple_cache_compute_and_write_stmt
+      OK
+      (reachable_locations_from_initial_env
+         simple_CT
+         (simple_heap (Int 41) (Int 0))
+         (simple_cache_env (Int 0)))
+      (simple_cache_env (Int (simple_derived [Int 41])))
+      h' /\
+    derived_int_cache_protocol
+      simple_CT
+      h'
+      simple_loc
+      simple_class
+      simple_abs_fields
+      simple_cache_field
+      simple_derived.
+Proof.
+  exists (update_field (simple_heap (Int 41) (Int 0)) simple_loc
+            simple_cache_field (Int (simple_derived [Int 41]))).
+  split.
+  - apply simple_cache_compute_and_write_eval.
+  - apply simple_update_known_cache_protocol.
+Qed.
