DerivedCacheIris.v
@@ -1,0 +1,252 @@
+From iris.bi Require Import bi.
+From iris.proofmode Require Import proofmode.
+
+Require Import Syntax Helpers Typing Bigstep DerivedCache.
+
+Section derived_cache_iris.
+  Context {PROP : bi}.
+
+  Definition derived_int_cache_protocolI
+      (CT : class_table) (h : heap) (loc : Loc) (C : class_name)
+      (abs_fields : list var) (cache_f : var)
+      (derived : list value -> nat) : PROP :=
+    ⌜derived_int_cache_protocol CT h loc C abs_fields cache_f derived⌝%I.
+
+  Definition field_readsI
+      (h : heap) (loc : Loc) (fields : list var) (vals : list value) : PROP :=
+    ⌜field_reads h loc fields vals⌝%I.
+
+  Lemma derived_int_cache_protocolI_intro :
+    forall CT h loc C abs_fields cache_f derived,
+      derived_int_cache_protocol CT h loc C abs_fields cache_f derived ->
+      ⊢ derived_int_cache_protocolI CT h loc C abs_fields cache_f derived.
+  Proof.
+    intros CT h loc C abs_fields cache_f derived Hprotocol.
+    iPureIntro.
+    exact Hprotocol.
+  Qed.
+
+  Lemma field_readsI_intro :
+    forall h loc fields vals,
+      field_reads h loc fields vals ->
+      ⊢ field_readsI h loc fields vals.
+  Proof.
+    intros h loc fields vals Hreads.
+    iPureIntro.
+    exact Hreads.
+  Qed.
+
+  Lemma eval_cache_field_write_establishes_protocolI :
+    forall CT rΓ h h' x y loc C abs_fields cache_f derived
+           abs_vals old_cache_v n o,
+      eval_stmt
+        OK
+        (reachable_locations_from_initial_env CT h rΓ)
+        CT rΓ h
+        (SFldWrite x cache_f y)
+        OK
+        (reachable_locations_from_initial_env CT h rΓ)
+        rΓ h' ->
+      runtime_getVal rΓ x = Some (Iot loc) ->
+      runtime_getVal rΓ y = Some (Int n) ->
+      runtime_getObj h loc = Some o ->
+      rctype (rt_type o) = C ->
+      final_fields CT C abs_fields ->
+      cache_field CT C cache_f ->
+      field_reads h loc abs_fields abs_vals ->
+      field_read h loc cache_f old_cache_v ->
+      n = derived abs_vals ->
+      n <> 0 ->
+      ⊢ derived_int_cache_protocolI CT h' loc C abs_fields cache_f derived.
+  Proof.
+    intros CT rΓ h h' x y loc C abs_fields cache_f derived
+           abs_vals old_cache_v n o
+           Heval Hx Hy Hobj HC Hfinals Hcache Hreads Hcache_read Hderived Hnz.
+    iPureIntro.
+    eapply eval_cache_field_write_establishes_protocol; eauto.
+  Qed.
+
+  Lemma eval_cache_field_write_preserves_final_readsI :
+    forall CT rΓ h h' x y loc C abs_fields cache_f abs_vals o,
+      eval_stmt
+        OK
+        (reachable_locations_from_initial_env CT h rΓ)
+        CT rΓ h
+        (SFldWrite x cache_f y)
+        OK
+        (reachable_locations_from_initial_env CT h rΓ)
+        rΓ h' ->
+      runtime_getVal rΓ x = Some (Iot loc) ->
+      runtime_getObj h loc = Some o ->
+      rctype (rt_type o) = C ->
+      final_fields CT C abs_fields ->
+      cache_field CT C cache_f ->
+      field_reads h loc abs_fields abs_vals ->
+      ⊢ field_readsI h' loc abs_fields abs_vals.
+  Proof.
+    intros CT rΓ h h' x y loc C abs_fields cache_f abs_vals o
+           Heval Hx Hobj HC Hfinals Hcache Hreads.
+    iPureIntro.
+    eapply eval_cache_field_write_preserves_final_reads; eauto.
+  Qed.
+
+  Lemma eval_int_compute_and_cache_write_soundI :
+    forall CT rΓ rΓ_mid h h' receiver tmp loc C abs_fields cache_f derived
+           abs_vals old_cache_v n o,
+      eval_stmt
+        OK
+        (reachable_locations_from_initial_env CT h rΓ)
+        CT rΓ h
+        (SVarAss tmp (EInt n))
+        OK
+        (reachable_locations_from_initial_env CT h rΓ)
+        rΓ_mid h ->
+      eval_stmt
+        OK
+        (reachable_locations_from_initial_env CT h rΓ_mid)
+        CT rΓ_mid h
+        (SFldWrite receiver cache_f tmp)
+        OK
+        (reachable_locations_from_initial_env CT h rΓ_mid)
+        rΓ_mid h' ->
+      runtime_getVal rΓ_mid receiver = Some (Iot loc) ->
+      runtime_getVal rΓ_mid tmp = Some (Int n) ->
+      runtime_getObj h loc = Some o ->
+      rctype (rt_type o) = C ->
+      final_fields CT C abs_fields ->
+      cache_field CT C cache_f ->
+      field_reads h loc abs_fields abs_vals ->
+      field_read h loc cache_f old_cache_v ->
+      n = derived abs_vals ->
+      n <> 0 ->
+      ⊢ field_readsI h' loc abs_fields abs_vals ∧
+        derived_int_cache_protocolI CT h' loc C abs_fields cache_f derived.
+  Proof.
+    intros CT rΓ rΓ_mid h h' receiver tmp loc C abs_fields cache_f derived
+           abs_vals old_cache_v n o
+           Hcompute Hwrite Hreceiver_mid Htmp_mid Hobj HC Hfinals Hcache
+           Hreads Hcache_read Hderived Hnz.
+    iPureIntro.
+    eapply eval_int_compute_and_cache_write_sound; eauto.
+  Qed.
+
+  Theorem derived_cache_update_immutabilityI :
+    forall CT sΓ mt rΓ rΓ_mid h h' receiver tmp loc C abs_fields cache_f
+           abs_vals n o,
+      wf_r_config CT sΓ rΓ h ->
+      stmt_typing CT sΓ mt (SVarAss tmp (EInt n)) sΓ ->
+      stmt_typing CT sΓ mt (SFldWrite receiver cache_f tmp) sΓ ->
+      eval_stmt
+        OK
+        (reachable_locations_from_initial_env CT h rΓ)
+        CT rΓ h
+        (SVarAss tmp (EInt n))
+        OK
+        (reachable_locations_from_initial_env CT h rΓ)
+        rΓ_mid h ->
+      eval_stmt
+        OK
+        (reachable_locations_from_initial_env CT h rΓ_mid)
+        CT rΓ_mid h
+        (SFldWrite receiver cache_f tmp)
+        OK
+        (reachable_locations_from_initial_env CT h rΓ_mid)
+        rΓ_mid h' ->
+      runtime_getVal rΓ_mid receiver = Some (Iot loc) ->
+      runtime_getObj h loc = Some o ->
+      rctype (rt_type o) = C ->
+      final_fields CT C abs_fields ->
+      cache_field CT C cache_f ->
+      field_reads h loc abs_fields abs_vals ->
+      ⊢ field_readsI h' loc abs_fields abs_vals.
+  Proof.
+    intros CT sΓ mt rΓ rΓ_mid h h' receiver tmp loc C abs_fields cache_f
+           abs_vals n o
+           Hwf Htype_compute Htype_write Hcompute Hwrite Hreceiver_mid Hobj
+           HC Hfinals Hcache Hreads.
+    iPureIntro.
+    eapply derived_cache_update_immutability; eauto.
+  Qed.
+
+  Theorem derived_cache_update_soundI :
+    forall CT sΓ mt rΓ rΓ_mid h h' receiver tmp loc C abs_fields cache_f
+           derived abs_vals old_cache_v n o,
+      wf_r_config CT sΓ rΓ h ->
+      stmt_typing CT sΓ mt (SVarAss tmp (EInt n)) sΓ ->
+      stmt_typing CT sΓ mt (SFldWrite receiver cache_f tmp) sΓ ->
+      eval_stmt
+        OK
+        (reachable_locations_from_initial_env CT h rΓ)
+        CT rΓ h
+        (SVarAss tmp (EInt n))
+        OK
+        (reachable_locations_from_initial_env CT h rΓ)
+        rΓ_mid h ->
+      eval_stmt
+        OK
+        (reachable_locations_from_initial_env CT h rΓ_mid)
+        CT rΓ_mid h
+        (SFldWrite receiver cache_f tmp)
+        OK
+        (reachable_locations_from_initial_env CT h rΓ_mid)
+        rΓ_mid h' ->
+      runtime_getVal rΓ_mid receiver = Some (Iot loc) ->
+      runtime_getVal rΓ_mid tmp = Some (Int n) ->
+      runtime_getObj h loc = Some o ->
+      rctype (rt_type o) = C ->
+      final_fields CT C abs_fields ->
+      cache_field CT C cache_f ->
+      field_reads h loc abs_fields abs_vals ->
+      field_read h loc cache_f old_cache_v ->
+      n = derived abs_vals ->
+      n <> 0 ->
+      ⊢ field_readsI h' loc abs_fields abs_vals ∧
+        derived_int_cache_protocolI CT h' loc C abs_fields cache_f derived.
+  Proof.
+    intros CT sΓ mt rΓ rΓ_mid h h' receiver tmp loc C abs_fields cache_f
+           derived abs_vals old_cache_v n o
+           Hwf Htype_compute Htype_write Hcompute Hwrite Hreceiver_mid Htmp_mid
+           Hobj HC Hfinals Hcache Hreads Hcache_read Hderived Hnz.
+    iPureIntro.
+    eapply derived_cache_update_sound; eauto.
+  Qed.
+
+  Theorem derived_cache_update_sequence_soundI :
+    forall CT sΓ mt rΓ rΓ_mid h h' receiver tmp loc C abs_fields cache_f
+           derived abs_vals old_cache_v n o,
+      wf_r_config CT sΓ rΓ h ->
+      stmt_typing CT sΓ mt (SVarAss tmp (EInt n)) sΓ ->
+      stmt_typing CT sΓ mt (SFldWrite receiver cache_f tmp) sΓ ->
+      rΓ_mid = set_vars rΓ (update tmp (Int n) (vars rΓ)) ->
+      reachable_locations_from_initial_env CT h rΓ_mid =
+        reachable_locations_from_initial_env CT h rΓ ->
+      eval_stmt
+        OK
+        (reachable_locations_from_initial_env CT h rΓ)
+        CT rΓ h
+        (SSeq (SVarAss tmp (EInt n)) (SFldWrite receiver cache_f tmp))
+        OK
+        (reachable_locations_from_initial_env CT h rΓ)
+        rΓ_mid h' ->
+      runtime_getVal rΓ_mid receiver = Some (Iot loc) ->
+      runtime_getVal rΓ_mid tmp = Some (Int n) ->
+      runtime_getObj h loc = Some o ->
+      rctype (rt_type o) = C ->
+      final_fields CT C abs_fields ->
+      cache_field CT C cache_f ->
+      field_reads h loc abs_fields abs_vals ->
+      field_read h loc cache_f old_cache_v ->
+      n = derived abs_vals ->
+      n <> 0 ->
+      ⊢ field_readsI h' loc abs_fields abs_vals ∧
+        derived_int_cache_protocolI CT h' loc C abs_fields cache_f derived.
+  Proof.
+    intros CT sΓ mt rΓ rΓ_mid h h' receiver tmp loc C abs_fields cache_f
+           derived abs_vals old_cache_v n o
+           Hwf Htype_compute Htype_write Hmid Hreach_stable Hseq
+           Hreceiver_mid Htmp_mid Hobj HC Hfinals Hcache Hreads Hcache_read
+           Hderived Hnz.
+    iPureIntro.
+    eapply derived_cache_update_sequence_sound; eauto.
+  Qed.
+End derived_cache_iris.
