DerivedCacheIrisExamples.v
@@ -1,0 +1,164 @@
+From iris.bi Require Import bi.
+From iris.proofmode Require Import proofmode.
+
+Require Import Syntax Helpers Bigstep DerivedCache DerivedCacheExamples
+  DerivedCacheIris.
+
+Section simple_derived_cache_iris_example.
+  Context {PROP : bi}.
+
+  Definition simple_cache_final_heap : heap :=
+    update_field (simple_heap (Int 41) (Int 0)) simple_loc
+      simple_cache_field (Int (simple_derived [Int 41])).
+
+  Lemma simple_cache_compute_and_write_protocolI :
+    ⊢ @derived_int_cache_protocolI PROP
+        simple_CT
+        simple_cache_final_heap
+        simple_loc
+        simple_class
+        simple_abs_fields
+        simple_cache_field
+        simple_derived.
+  Proof.
+    apply derived_int_cache_protocolI_intro.
+    unfold simple_cache_final_heap.
+    apply simple_update_known_cache_protocol.
+  Qed.
+
+  Lemma simple_cache_write_preserves_final_readsI :
+    ⊢ @field_readsI PROP
+        simple_cache_final_heap
+        simple_loc
+        simple_abs_fields
+        [Int 41].
+  Proof.
+    apply field_readsI_intro.
+    unfold simple_cache_final_heap.
+    eapply update_cache_field_preserves_final_field_reads
+      with
+        (CT := simple_CT)
+        (C := simple_class)
+        (o := simple_obj (Int 41) (Int 0)).
+    - apply simple_object_lookup.
+    - reflexivity.
+    - apply simple_cache_field_assignable.
+    - apply simple_final_fields.
+    - apply simple_field_reads.
+    - reflexivity.
+  Qed.
+
+  Lemma simple_cache_compute_and_write_eval_protocolI :
+    exists h',
+      eval_stmt
+        OK
+        (reachable_locations_from_initial_env
+           simple_CT
+           (simple_heap (Int 41) (Int 0))
+           (simple_cache_env (Int 0)))
+        simple_CT
+        (simple_cache_env (Int 0))
+        (simple_heap (Int 41) (Int 0))
+        simple_cache_compute_and_write_stmt
+        OK
+        (reachable_locations_from_initial_env
+           simple_CT
+           (simple_heap (Int 41) (Int 0))
+           (simple_cache_env (Int 0)))
+        (simple_cache_env (Int (simple_derived [Int 41])))
+      h' /\
+      (⊢ @derived_int_cache_protocolI PROP
+            simple_CT
+            h'
+            simple_loc
+            simple_class
+            simple_abs_fields
+            simple_cache_field
+            simple_derived).
+  Proof.
+    exists simple_cache_final_heap.
+    split.
+    - unfold simple_cache_final_heap.
+      apply simple_cache_compute_and_write_eval.
+    - apply simple_cache_compute_and_write_protocolI.
+  Qed.
+
+  Lemma simple_cache_compute_and_write_eval_soundI :
+    exists h',
+      eval_stmt
+        OK
+        (reachable_locations_from_initial_env
+           simple_CT
+           (simple_heap (Int 41) (Int 0))
+           (simple_cache_env (Int 0)))
+        simple_CT
+        (simple_cache_env (Int 0))
+        (simple_heap (Int 41) (Int 0))
+        simple_cache_compute_and_write_stmt
+        OK
+        (reachable_locations_from_initial_env
+           simple_CT
+           (simple_heap (Int 41) (Int 0))
+           (simple_cache_env (Int 0)))
+        (simple_cache_env (Int (simple_derived [Int 41])))
+        h' /\
+      (⊢ @field_readsI PROP h' simple_loc simple_abs_fields [Int 41]) /\
+      (⊢ @derived_int_cache_protocolI PROP
+            simple_CT
+            h'
+            simple_loc
+            simple_class
+            simple_abs_fields
+            simple_cache_field
+            simple_derived).
+  Proof.
+    exists simple_cache_final_heap.
+    repeat split.
+    - unfold simple_cache_final_heap.
+      apply simple_cache_compute_and_write_eval.
+    - apply simple_cache_write_preserves_final_readsI.
+    - apply simple_cache_compute_and_write_protocolI.
+  Qed.
+
+  Lemma simple_cache_compute_and_write_component_soundI :
+    ⊢ @field_readsI PROP
+        simple_cache_final_heap
+        simple_loc
+        simple_abs_fields
+        [Int 41] ∧
+      @derived_int_cache_protocolI PROP
+        simple_CT
+        simple_cache_final_heap
+        simple_loc
+        simple_class
+        simple_abs_fields
+        simple_cache_field
+        simple_derived.
+  Proof.
+    unfold simple_cache_final_heap.
+    eapply eval_int_compute_and_cache_write_soundI
+      with
+        (CT := simple_CT)
+        (rΓ := simple_cache_env (Int 0))
+        (rΓ_mid := simple_cache_env (Int (simple_derived [Int 41])))
+        (receiver := 0)
+        (tmp := simple_cache_tmp_var)
+        (C := simple_class)
+        (abs_vals := [Int 41])
+        (old_cache_v := Int 0)
+        (n := simple_derived [Int 41])
+        (o := simple_obj (Int 41) (Int 0)).
+    - apply simple_assign_literal_eval.
+    - apply simple_cache_write_eval.
+    - unfold simple_cache_env, simple_loc. reflexivity.
+    - unfold simple_cache_env, simple_cache_tmp_var. reflexivity.
+    - apply simple_object_lookup.
+    - reflexivity.
+    - apply simple_final_fields.
+    - apply simple_cache_field_assignable.
+    - apply simple_field_reads.
+    - apply simple_cache_read.
+    - unfold simple_derived. reflexivity.
+    - unfold simple_derived. lia.
+  Qed.
+End simple_derived_cache_iris_example.
