StringCacheIris.v
@@ -1,0 +1,424 @@
+From Stdlib Require Import ZArith.
+
+From iris.proofmode Require Import proofmode.
+From iris.heap_lang Require Import proofmode notation.
+From iris.heap_lang.lib Require Import spawn.
+From iris.base_logic.lib Require Import invariants.
+
+Open Scope Z_scope.
+
+(* This file is an ordinary Iris/heap_lang wrapper for the cache idea. It is
+   intentionally sequentially consistent: heap_lang gives interleaving
+   concurrency with atomic heap operations, not Java weak-memory races. *)
+
+Definition deterministic_hash (v c : Z) : Z :=
+  v + 31 * c.
+
+Definition CacheOK (H h : Z) (hashIsZero : bool) : Prop :=
+  (h = 0 \/ h = H) /\
+  (H = 0 \/ hashIsZero = false).
+
+Definition mk_string_obj : val :=
+  λ: "value" "coder",
+    let: "hash" := ref #0 in
+    let: "hashIsZero" := ref #false in
+    ("value", "coder", "hash", "hashIsZero").
+
+Definition hashCode_store_nonzero : val :=
+  λ: "o",
+    let: "value" := Fst (Fst (Fst "o")) in
+    let: "coder" := Snd (Fst (Fst "o")) in
+    let: "hash" := Snd (Fst "o") in
+    let: "computed" := "value" + (#31 * "coder") in
+    "hash" <- "computed";;
+    "computed".
+
+Definition hashCode_local_copy_nonzero : val :=
+  λ: "o",
+    let: "value" := Fst (Fst (Fst "o")) in
+    let: "coder" := Snd (Fst (Fst "o")) in
+    let: "hash" := Snd (Fst "o") in
+    let: "h" := !"hash" in
+    if: "h" = #0 then
+      let: "computed" := "value" + (#31 * "coder") in
+      "hash" <- "computed";;
+      "computed"
+    else
+      "h".
+
+Definition hashCode_local_copy_zero : val :=
+  λ: "o",
+    let: "value" := Fst (Fst (Fst "o")) in
+    let: "coder" := Snd (Fst (Fst "o")) in
+    let: "hash" := Snd (Fst "o") in
+    let: "hashIsZero" := Snd "o" in
+    let: "h" := !"hash" in
+    if: "h" = #0 then
+      let: "computed" := "value" + (#31 * "coder") in
+      if: "computed" = #0 then
+        "hashIsZero" <- #true;;
+        "computed"
+      else
+        "hash" <- "computed";;
+        "computed"
+    else
+      "h".
+
+Definition hashCode_local_copy : val := hashCode_local_copy_zero.
+
+Definition hashCode_fork2 : val :=
+  λ: "o",
+    Fork (hashCode_local_copy "o");;
+    Fork (hashCode_local_copy "o");;
+    #().
+
+Definition hashCode_spawn2_join : val :=
+  λ: "o",
+    let: "h1" := spawn.spawn (λ: <>, hashCode_local_copy "o") in
+    let: "h2" := spawn.spawn (λ: <>, hashCode_local_copy "o") in
+    let: "r1" := spawn.join "h1" in
+    let: "r2" := spawn.join "h2" in
+    ("r1", "r2").
+
+Section proofs.
+  Context `{!heapGS Σ}.
+
+  Definition ImmString (N : namespace) (o : val) (v c : Z) : iProp Σ :=
+    ∃ (hash hashIsZero : loc),
+      ⌜o = (#v, #c, #hash, #hashIsZero)%V⌝ ∗
+      inv N (∃ (h : Z) (z : bool),
+        hash ↦ #h ∗
+        hashIsZero ↦ #z ∗
+        ⌜CacheOK (deterministic_hash v c) h z⌝).
+
+  Global Instance ImmString_persistent N o v c :
+    Persistent (ImmString N o v c).
+  Proof. apply _. Qed.
+
+  Lemma mk_string_obj_spec N v c :
+    {{{ True }}}
+      mk_string_obj #v #c
+    {{{ o, RET o; ImmString N o v c }}}.
+  Proof.
+    iIntros (Φ) "_ HΦ".
+    rewrite /mk_string_obj.
+    wp_pures.
+    wp_alloc hash as "Hhash".
+    wp_pures.
+    wp_alloc hashIsZero as "HhashIsZero".
+    wp_pures.
+    iMod (inv_alloc N _ (∃ (h : Z) (z : bool),
+            hash ↦ #h ∗
+            hashIsZero ↦ #z ∗
+            ⌜CacheOK (deterministic_hash v c) h z⌝)%I
+          with "[Hhash HhashIsZero]") as "#Hinv".
+    {
+      iNext.
+      iExists 0, false.
+      iFrame.
+      iPureIntro.
+      split; [left | right]; reflexivity.
+    }
+    iModIntro.
+    iApply "HΦ".
+    iExists hash, hashIsZero.
+    iSplit; [done | iExact "Hinv"].
+  Qed.
+
+  Lemma hashCode_store_nonzero_spec N o v c :
+    deterministic_hash v c ≠ 0 ->
+    {{{ ImmString N o v c }}}
+      hashCode_store_nonzero o
+    {{{ RET #(deterministic_hash v c); ImmString N o v c }}}.
+  Proof.
+    iIntros (Hnz Φ) "Himm HΦ".
+    iDestruct "Himm" as (hash hashIsZero ->) "#Hinv".
+    rewrite /hashCode_store_nonzero /deterministic_hash.
+    wp_pures.
+    wp_bind (#hash <- #(v + 31 * c))%E.
+    iInv N as (h z) "(>Hhash & >HhashIsZero & >%Hok)" "Hclose".
+    wp_store.
+    iMod ("Hclose" with "[Hhash HhashIsZero]") as "_".
+    {
+      iNext.
+      iExists (v + 31 * c), z.
+      iFrame.
+      iPureIntro.
+      destruct Hok as [_ Hz].
+      split.
+      - right. reflexivity.
+      - destruct Hz as [Hzero | Hzfalse]; [contradiction | right; exact Hzfalse].
+    }
+    iModIntro.
+    wp_pures.
+    iApply "HΦ".
+    iModIntro.
+    iExists hash, hashIsZero.
+    iSplit; [done | iExact "Hinv"].
+  Qed.
+
+  Lemma hashCode_local_copy_nonzero_spec N o v c :
+    deterministic_hash v c ≠ 0 ->
+    {{{ ImmString N o v c }}}
+      hashCode_local_copy_nonzero o
+    {{{ RET #(deterministic_hash v c); ImmString N o v c }}}.
+  Proof.
+    iIntros (Hnz Φ) "Himm HΦ".
+    unfold deterministic_hash in Hnz.
+    iDestruct "Himm" as (hash hashIsZero ->) "#Hinv".
+    rewrite /hashCode_local_copy_nonzero /deterministic_hash.
+    wp_pures.
+    wp_bind (! #hash)%E.
+    iInv N as (h z) "(>Hhash & >HhashIsZero & >%Hok)" "Hclose".
+    wp_load.
+    iMod ("Hclose" with "[Hhash HhashIsZero]") as "_".
+    {
+      iNext.
+      iExists h, z.
+      iFrame.
+      done.
+    }
+    iModIntro.
+    destruct Hok as [[Hh_zero | Hh_hash] Hz].
+    - subst h.
+      wp_pures.
+      wp_bind (#hash <- #(v + 31 * c))%E.
+      iInv N as (h2 z2) "(>Hhash & >HhashIsZero & >%Hok)" "Hclose".
+      wp_store.
+      iMod ("Hclose" with "[Hhash HhashIsZero]") as "_".
+      {
+        iNext.
+        iExists (v + 31 * c), z2.
+        iFrame.
+        iPureIntro.
+        destruct Hok as [_ Hz2].
+        split.
+        + right. reflexivity.
+        + destruct Hz2 as [Hzero | Hzfalse];
+            [contradiction | right; exact Hzfalse].
+      }
+      iModIntro.
+      wp_pures.
+      iApply "HΦ".
+      iModIntro.
+      iExists hash, hashIsZero.
+      iSplit; [done | iExact "Hinv"].
+    - subst h.
+      wp_pures.
+      rewrite bool_decide_false.
+      2: { intros Heq. inversion Heq. apply Hnz. exact H0. }
+      wp_pures.
+      iApply "HΦ".
+      iModIntro.
+      iExists hash, hashIsZero.
+      iSplit; [done | iExact "Hinv"].
+  Qed.
+
+  Lemma hashCode_local_copy_zero_spec N o v c :
+    deterministic_hash v c = 0 ->
+    {{{ ImmString N o v c }}}
+      hashCode_local_copy_zero o
+    {{{ RET #0; ImmString N o v c }}}.
+  Proof.
+    iIntros (Hzero Φ) "Himm HΦ".
+    unfold deterministic_hash in Hzero.
+    iDestruct "Himm" as (hash hashIsZero ->) "#Hinv".
+    rewrite /hashCode_local_copy_zero /deterministic_hash.
+    wp_pures.
+    wp_bind (! #hash)%E.
+    iInv N as (h z) "(>Hhash & >HhashIsZero & >%Hok)" "Hclose".
+    wp_load.
+    iMod ("Hclose" with "[Hhash HhashIsZero]") as "_".
+    {
+      iNext.
+      iExists h, z.
+      iFrame.
+      done.
+    }
+    iModIntro.
+    destruct Hok as [[Hh_zero | Hh_hash] _].
+    - subst h.
+      wp_pures.
+      rewrite bool_decide_true; last (rewrite Hzero; reflexivity).
+      wp_pures.
+      wp_bind (#hashIsZero <- #true)%E.
+      iInv N as (h2 z2) "(>Hhash & >HhashIsZero & >%Hok)" "Hclose".
+      wp_store.
+      iMod ("Hclose" with "[Hhash HhashIsZero]") as "_".
+      {
+        iNext.
+        iExists h2, true.
+        iFrame.
+        iPureIntro.
+        destruct Hok as [Hh_ok _].
+        split; [exact Hh_ok | left; exact Hzero].
+      }
+      iModIntro.
+      wp_pures.
+      replace (#(v + 31 * c))%V with (#0)%V
+        by (rewrite Hzero; reflexivity).
+      iApply "HΦ".
+      iModIntro.
+      iExists hash, hashIsZero.
+      iSplit; [done | rewrite /deterministic_hash Hzero; iExact "Hinv"].
+    - rewrite Hzero in Hh_hash.
+      subst h.
+      wp_pures.
+      rewrite bool_decide_true; last (rewrite Hzero; reflexivity).
+      wp_pures.
+      wp_bind (#hashIsZero <- #true)%E.
+      iInv N as (h2 z2) "(>Hhash & >HhashIsZero & >%Hok)" "Hclose".
+      wp_store.
+      iMod ("Hclose" with "[Hhash HhashIsZero]") as "_".
+      {
+        iNext.
+        iExists h2, true.
+        iFrame.
+        iPureIntro.
+        destruct Hok as [Hh_ok _].
+        split; [exact Hh_ok | left; exact Hzero].
+      }
+      iModIntro.
+      wp_pures.
+      replace (#(v + 31 * c))%V with (#0)%V
+        by (rewrite Hzero; reflexivity).
+      iApply "HΦ".
+      iModIntro.
+      iExists hash, hashIsZero.
+      iSplit; [done | rewrite /deterministic_hash Hzero; iExact "Hinv"].
+  Qed.
+
+  Lemma hashCode_local_copy_nonzero_full_spec N o v c :
+    deterministic_hash v c ≠ 0 ->
+    {{{ ImmString N o v c }}}
+      hashCode_local_copy o
+    {{{ RET #(deterministic_hash v c); ImmString N o v c }}}.
+  Proof.
+    iIntros (Hnz Φ) "Himm HΦ".
+    unfold deterministic_hash in Hnz.
+    iDestruct "Himm" as (hash hashIsZero ->) "#Hinv".
+    rewrite /hashCode_local_copy /hashCode_local_copy_zero /deterministic_hash.
+    wp_pures.
+    wp_bind (! #hash)%E.
+    iInv N as (h z) "(>Hhash & >HhashIsZero & >%Hok)" "Hclose".
+    wp_load.
+    iMod ("Hclose" with "[Hhash HhashIsZero]") as "_".
+    {
+      iNext.
+      iExists h, z.
+      iFrame.
+      done.
+    }
+    iModIntro.
+    destruct Hok as [[Hh_zero | Hh_hash] Hz].
+    - subst h.
+      wp_pures.
+      rewrite bool_decide_false.
+      2: { intros Heq. inversion Heq. apply Hnz. exact H0. }
+      wp_pures.
+      wp_bind (#hash <- #(v + 31 * c))%E.
+      iInv N as (h2 z2) "(>Hhash & >HhashIsZero & >%Hok)" "Hclose".
+      wp_store.
+      iMod ("Hclose" with "[Hhash HhashIsZero]") as "_".
+      {
+        iNext.
+        iExists (v + 31 * c), z2.
+        iFrame.
+        iPureIntro.
+        destruct Hok as [_ Hz2].
+        split.
+        + right. reflexivity.
+        + destruct Hz2 as [Hzero | Hzfalse];
+            [contradiction | right; exact Hzfalse].
+      }
+      iModIntro.
+      wp_pures.
+      iApply "HΦ".
+      iModIntro.
+      iExists hash, hashIsZero.
+      iSplit; [done | iExact "Hinv"].
+    - subst h.
+      wp_pures.
+      rewrite bool_decide_false.
+      2: { intros Heq. inversion Heq. apply Hnz. exact H0. }
+      wp_pures.
+      iApply "HΦ".
+      iModIntro.
+      iExists hash, hashIsZero.
+      iSplit; [done | iExact "Hinv"].
+  Qed.
+
+  Lemma hashCode_local_copy_spec N o v c :
+    {{{ ImmString N o v c }}}
+      hashCode_local_copy o
+    {{{ RET #(deterministic_hash v c); ImmString N o v c }}}.
+  Proof.
+    destruct (Z.eq_dec (deterministic_hash v c) 0) as [Hzero | Hnz].
+    - rewrite /hashCode_local_copy.
+      replace (#(deterministic_hash v c))%V with #0%V
+        by (rewrite Hzero; reflexivity).
+      apply hashCode_local_copy_zero_spec.
+      exact Hzero.
+    - apply hashCode_local_copy_nonzero_full_spec.
+      exact Hnz.
+  Qed.
+
+  Lemma hashCode_fork2_spec N o v c :
+    {{{ ImmString N o v c }}}
+      hashCode_fork2 o
+    {{{ RET #(); ImmString N o v c }}}.
+  Proof.
+    iIntros (Φ) "#Himm HΦ".
+    rewrite /hashCode_fork2.
+    wp_pures.
+    wp_apply wp_fork.
+    - wp_apply (hashCode_local_copy_spec with "Himm").
+      iIntros "_".
+      done.
+    - wp_seq.
+      wp_apply wp_fork.
+      + wp_apply (hashCode_local_copy_spec with "Himm").
+        iIntros "_".
+        done.
+      + wp_seq.
+        iApply "HΦ".
+        iExact "Himm".
+  Qed.
+
+  Lemma hashCode_spawn2_join_spec `{!spawnG Σ} N (Nspawn : namespace) o v c :
+    {{{ ImmString N o v c }}}
+      hashCode_spawn2_join o
+    {{{ RET (#(deterministic_hash v c), #(deterministic_hash v c))%V;
+        ImmString N o v c }}}.
+  Proof.
+    iIntros (Φ) "#Himm HΦ".
+    rewrite /hashCode_spawn2_join.
+    wp_pures.
+    wp_apply (spawn_spec Nspawn
+      (fun r => ⌜r = #(deterministic_hash v c)⌝%I) with "[Himm]").
+    - wp_pures.
+      wp_apply (hashCode_local_copy_spec with "Himm").
+      iIntros "_".
+      done.
+    - iIntros (h1) "Hh1".
+      wp_pures.
+      wp_apply (spawn_spec Nspawn
+        (fun r => ⌜r = #(deterministic_hash v c)⌝%I) with "[Himm]").
+      + wp_pures.
+        wp_apply (hashCode_local_copy_spec with "Himm").
+        iIntros "_".
+        done.
+      + iIntros (h2) "Hh2".
+        wp_pures.
+        wp_apply (join_spec with "Hh1").
+        iIntros (r1) "%Hr1".
+        subst r1.
+        wp_pures.
+        wp_apply (join_spec with "Hh2").
+        iIntros (r2) "%Hr2".
+        subst r2.
+        wp_pures.
+        iApply "HΦ".
+        iExact "Himm".
+  Qed.
+End proofs.
