WeakPico.v
@@ -1,0 +1,231 @@
+Require Import Syntax Helpers Bigstep DerivedCache ConcurrentPico.
+
+From Stdlib Require Import List.
+Import ListNotations.
+
+(* A first weak-memory-facing PICO model.
+
+   Unlike [ConcurrentPico], this file makes read observations explicit.  A weak
+   execution may propose a cache write computed from observed abstract-field
+   values.  We accept the write only when those observations are coherent with
+   the final-field values in the shared heap at commit time.
+
+   This is still not the full Java memory model.  It is the next artifact layer:
+   it separates candidate weak executions from the safety condition needed for
+   derived-cache soundness.
+*)
+
+Record weak_cache_write := mkWeakCacheWrite {
+  weak_loc : Loc;
+  weak_class : class_name;
+  weak_abs_fields : list var;
+  weak_cache_field : var;
+  weak_observed_abs_vals : list value;
+  weak_observed_old_cache : value;
+  weak_written_cache_n : nat;
+}.
+
+Definition weak_cache_write_coherent
+    (CT : class_table) (h : heap) (derived : list value -> nat)
+    (e : weak_cache_write) : Prop :=
+  exists o,
+    runtime_getObj h (weak_loc e) = Some o /\
+    rctype (rt_type o) = weak_class e /\
+    final_fields CT (weak_class e) (weak_abs_fields e) /\
+    cache_field CT (weak_class e) (weak_cache_field e) /\
+    field_reads h (weak_loc e) (weak_abs_fields e)
+      (weak_observed_abs_vals e) /\
+    field_read h (weak_loc e) (weak_cache_field e)
+      (weak_observed_old_cache e) /\
+    weak_written_cache_n e = derived (weak_observed_abs_vals e) /\
+    weak_written_cache_n e <> 0.
+
+Definition weak_cache_write_commit
+    (h h' : heap) (e : weak_cache_write) : Prop :=
+  h' =
+    update_field h (weak_loc e) (weak_cache_field e)
+      (Int (weak_written_cache_n e)).
+
+Definition weak_candidate_cache_transition
+    (h h' : heap) (e : weak_cache_write) : Prop :=
+  weak_cache_write_commit h h' e.
+
+Definition weak_accepts_cache_transition
+    (CT : class_table) (h h' : heap) (derived : list value -> nat)
+    (e : weak_cache_write) : Prop :=
+  weak_candidate_cache_transition h h' e /\
+  weak_cache_write_coherent CT h derived e.
+
+Definition weak_rejects_cache_transition
+    (CT : class_table) (h h' : heap) (derived : list value -> nat)
+    (e : weak_cache_write) : Prop :=
+  not (weak_accepts_cache_transition CT h h' derived e).
+
+Lemma weak_accepts_preserves_protocol :
+  forall CT h h' derived e,
+    weak_accepts_cache_transition CT h h' derived e ->
+    derived_int_cache_protocol
+      CT h'
+      (weak_loc e)
+      (weak_class e)
+      (weak_abs_fields e)
+      (weak_cache_field e)
+      derived.
+Proof.
+  intros CT h h' derived e [Hcommit Hcoherent].
+  destruct Hcoherent as
+    [o [Hobj [HC [Hfinals [Hcache [Hreads
+      [Hcache_read [Hderived Hnz]]]]]]]].
+  unfold weak_candidate_cache_transition, weak_cache_write_commit in Hcommit.
+  eapply update_known_int_cache_preserves_protocol; eauto.
+Qed.
+
+Theorem weak_rejects_protocol_break :
+  forall CT h h' derived e,
+    weak_candidate_cache_transition h h' e ->
+    not
+      (derived_int_cache_protocol
+        CT h'
+        (weak_loc e)
+        (weak_class e)
+        (weak_abs_fields e)
+        (weak_cache_field e)
+        derived) ->
+    weak_rejects_cache_transition CT h h' derived e.
+Proof.
+  intros CT h h' derived e Hcandidate Hbreak Haccepted.
+  apply Hbreak.
+  eapply weak_accepts_preserves_protocol; eauto.
+Qed.
+
+Definition weak_event_matches_sc_transition
+    (CT : class_table) (h h' : heap) (derived : list value -> nat)
+    (e : weak_cache_write) : Prop :=
+  weak_accepts_cache_transition CT h h' derived e.
+
+Theorem weak_accepted_event_is_sc_cache_safe :
+  forall CT h h' derived e,
+    weak_event_matches_sc_transition CT h h' derived e ->
+    sc_accepts_cache_transition
+      CT h h'
+      (weak_loc e)
+      (weak_class e)
+      (weak_abs_fields e)
+      (weak_cache_field e)
+      derived.
+Proof.
+  intros CT h h' derived e [Hcommit Hcoherent].
+  destruct Hcoherent as
+    [o [Hobj [HC [_ [_ [Hreads
+      [Hcache_read [Hderived Hnz]]]]]]]].
+  unfold weak_candidate_cache_transition, weak_cache_write_commit in Hcommit.
+  eapply sc_accepts_derived_cache_write; eauto.
+Qed.
+
+Definition weak_event_targets_cache
+    (loc : Loc) (C : class_name) (abs_fields : list var) (cache_f : var)
+    (e : weak_cache_write) : Prop :=
+  weak_loc e = loc /\
+  weak_class e = C /\
+  weak_abs_fields e = abs_fields /\
+  weak_cache_field e = cache_f.
+
+Inductive weak_execution
+    (CT : class_table) (derived : list value -> nat) :
+    heap -> list weak_cache_write -> heap -> Prop :=
+  | WE_Nil : forall h,
+      weak_execution CT derived h [] h
+  | WE_Cons : forall h h' h'' e es,
+      weak_accepts_cache_transition CT h h' derived e ->
+      weak_execution CT derived h' es h'' ->
+      weak_execution CT derived h (e :: es) h''.
+
+Inductive weak_candidate_execution :
+    heap -> list weak_cache_write -> heap -> Prop :=
+  | WCE_Nil : forall h,
+      weak_candidate_execution h [] h
+  | WCE_Cons : forall h h' h'' e es,
+      weak_candidate_cache_transition h h' e ->
+      weak_candidate_execution h' es h'' ->
+      weak_candidate_execution h (e :: es) h''.
+
+Definition weak_rejects_execution
+    (CT : class_table) (derived : list value -> nat)
+    (h : heap) (events : list weak_cache_write) (h' : heap) : Prop :=
+  weak_candidate_execution h events h' /\
+  not (weak_execution CT derived h events h').
+
+Lemma weak_candidate_cache_transition_deterministic :
+  forall h h1 h2 e,
+    weak_candidate_cache_transition h h1 e ->
+    weak_candidate_cache_transition h h2 e ->
+    h1 = h2.
+Proof.
+  intros h h1 h2 e H1 H2.
+  unfold weak_candidate_cache_transition, weak_cache_write_commit in *.
+  congruence.
+Qed.
+
+Theorem weak_rejects_execution_at_head :
+  forall CT derived h h1 h' e es,
+    weak_candidate_cache_transition h h1 e ->
+    weak_rejects_cache_transition CT h h1 derived e ->
+    weak_candidate_execution h1 es h' ->
+    weak_rejects_execution CT derived h (e :: es) h'.
+Proof.
+  intros CT derived h h1 h' e es Hcandidate Hreject Htail.
+  split.
+  - eapply WCE_Cons; eauto.
+  - intro Haccepted_execution.
+    inversion Haccepted_execution as
+      [|h0 h_acc h_final e0 es0 Haccepted_head Haccepted_tail]; subst.
+    destruct Haccepted_head as [Haccepted_candidate Hcoherent].
+    assert (h_acc = h1).
+    {
+      eapply weak_candidate_cache_transition_deterministic; eauto.
+    }
+    subst h_acc.
+    apply Hreject.
+    split; assumption.
+Qed.
+
+Lemma weak_accepts_preserves_cache_state_for_target :
+  forall CT h h' loc C abs_fields cache_f derived e,
+    weak_event_targets_cache loc C abs_fields cache_f e ->
+    weak_accepts_cache_transition CT h h' derived e ->
+    concurrent_derived_cache_state CT h loc C abs_fields cache_f derived ->
+    concurrent_derived_cache_state CT h' loc C abs_fields cache_f derived.
+Proof.
+  intros CT h h' loc C abs_fields cache_f derived e
+         [Hloc [HC_target [Habs Hcache_target]]] Haccepted _.
+  destruct Haccepted as [Hcommit Hcoherent].
+  destruct Hcoherent as
+    [o [Hobj [HC [Hfinals [Hcache [Hreads
+      [Hcache_read [Hderived Hnz]]]]]]]].
+  unfold weak_candidate_cache_transition, weak_cache_write_commit in Hcommit.
+  subst h'.
+  subst loc C abs_fields cache_f.
+  exists (set_fields_map o
+    (update (weak_cache_field e) (Int (weak_written_cache_n e))
+      (fields_map o))).
+  split.
+  - eapply update_cache_field_preserves_runtime_type; eauto.
+  - split.
+    + simpl. exact HC.
+    + eapply update_known_int_cache_preserves_protocol; eauto.
+Qed.
+
+Theorem weak_execution_preserves_cache_state_for_target :
+  forall CT h h' events loc C abs_fields cache_f derived,
+    weak_execution CT derived h events h' ->
+    Forall (weak_event_targets_cache loc C abs_fields cache_f) events ->
+    concurrent_derived_cache_state CT h loc C abs_fields cache_f derived ->
+    concurrent_derived_cache_state CT h' loc C abs_fields cache_f derived.
+Proof.
+  intros CT h h' events loc C abs_fields cache_f derived Hexec Htargets Hstate.
+  induction Hexec as [h0 | h0 h1 h2 e es Haccepted Hexec_tail IH].
+  - exact Hstate.
+  - inversion Htargets as [|? ? Htarget Htargets_tail]; subst.
+    apply IH; [exact Htargets_tail |].
+    eapply weak_accepts_preserves_cache_state_for_target; eauto.
+Qed.
