WeakPicoExamples.v
@@ -1,0 +1,520 @@
+Require Import Syntax Helpers Typing Bigstep DerivedCache DerivedCacheExamples.
+Require Import ConcurrentPico WeakPico ConcurrentPicoExamples.
+
+From Stdlib Require Import List Lia.
+Import ListNotations.
+
+Definition simple_weak_coherent_event : weak_cache_write :=
+  mkWeakCacheWrite
+    simple_loc
+    simple_class
+    simple_abs_fields
+    simple_cache_field
+    [Int 41]
+    (Int 0)
+    (simple_derived [Int 41]).
+
+Definition simple_weak_incoherent_event : weak_cache_write :=
+  mkWeakCacheWrite
+    simple_loc
+    simple_class
+    simple_abs_fields
+    simple_cache_field
+    [Int 99]
+    (Int 0)
+    (simple_derived [Int 99]).
+
+Definition simple_weak_coherent_rewrite_event : weak_cache_write :=
+  mkWeakCacheWrite
+    simple_loc
+    simple_class
+    simple_abs_fields
+    simple_cache_field
+    [Int 41]
+    (Int (simple_derived [Int 41]))
+    (simple_derived [Int 41]).
+
+Definition simple_weak_bad_heap : heap :=
+  update_field
+    simple_sc_initial_heap
+    simple_loc
+    simple_cache_field
+    (Int (simple_derived [Int 99])).
+
+Lemma simple_weak_accepts_coherent_cache_write :
+  weak_accepts_cache_transition
+    simple_CT
+    simple_sc_initial_heap
+    simple_sc_cache_written_heap
+    simple_derived
+    simple_weak_coherent_event.
+Proof.
+  split.
+  - reflexivity.
+  - exists (simple_obj (Int 41) (Int 0)).
+    split; [reflexivity |].
+    split; [reflexivity |].
+    split; [apply simple_final_fields |].
+    split; [apply simple_cache_field_assignable |].
+    split; [apply simple_field_reads |].
+    split; [apply simple_cache_read |].
+    split; [reflexivity |].
+    unfold simple_derived. discriminate.
+Qed.
+
+Lemma simple_weak_bad_heap_not_protocol :
+  not
+    (derived_int_cache_protocol
+      simple_CT
+      simple_weak_bad_heap
+      simple_loc
+      simple_class
+      simple_abs_fields
+      simple_cache_field
+      simple_derived).
+Proof.
+  intro Hprotocol.
+  destruct Hprotocol as
+    [abs_vals [cache_v [_ [_ [Hreads [Hcache_read Hcache_value]]]]]].
+  unfold simple_weak_bad_heap, simple_sc_initial_heap, simple_heap, simple_obj,
+    simple_loc, simple_abs_fields, simple_cache_field in *.
+  simpl in Hreads.
+  inversion Hreads as [|? ? abs_v abs_tail Hread_abs Hreads_tail]; subst.
+  inversion Hreads_tail; subst.
+  destruct Hread_abs as [o_abs [Hobj_abs Hfield_abs]].
+  simpl in Hobj_abs.
+  inversion Hobj_abs; subst.
+  simpl in Hfield_abs.
+  inversion Hfield_abs; subst.
+  destruct Hcache_read as [o_cache [Hobj_cache Hfield_cache]].
+  simpl in Hobj_cache.
+  inversion Hobj_cache; subst.
+  simpl in Hfield_cache.
+  inversion Hfield_cache; subst.
+  simpl in Hcache_value.
+  destruct Hcache_value as [Hunknown | Hknown].
+  - discriminate.
+  - destruct Hknown as [n [Hcache_eq [Hderived Hnz]]].
+    assert (Hn : n = simple_derived [Int 99]).
+    { inversion Hcache_eq. reflexivity. }
+    simpl in Hderived.
+    simpl in Hn.
+    lia.
+Qed.
+
+Lemma simple_weak_rejects_incoherent_cache_write :
+  weak_rejects_cache_transition
+    simple_CT
+    simple_sc_initial_heap
+    simple_weak_bad_heap
+    simple_derived
+    simple_weak_incoherent_event.
+Proof.
+  eapply weak_rejects_protocol_break.
+  - reflexivity.
+  - apply simple_weak_bad_heap_not_protocol.
+Qed.
+
+Lemma simple_weak_coherent_event_targets_cache :
+  weak_event_targets_cache
+    simple_loc
+    simple_class
+    simple_abs_fields
+    simple_cache_field
+    simple_weak_coherent_event.
+Proof.
+  repeat split; reflexivity.
+Qed.
+
+Lemma simple_weak_coherent_rewrite_event_targets_cache :
+  weak_event_targets_cache
+    simple_loc
+    simple_class
+    simple_abs_fields
+    simple_cache_field
+    simple_weak_coherent_rewrite_event.
+Proof.
+  repeat split; reflexivity.
+Qed.
+
+Lemma simple_sc_cache_written_heap_stable_write :
+  weak_accepts_cache_transition
+    simple_CT
+    simple_sc_cache_written_heap
+    simple_sc_cache_written_heap
+    simple_derived
+    simple_weak_coherent_rewrite_event.
+Proof.
+  split.
+  - reflexivity.
+  - unfold simple_sc_cache_written_heap, simple_sc_initial_heap,
+      simple_weak_coherent_rewrite_event.
+    simpl.
+    exists (simple_obj (Int 41) (Int (simple_derived [Int 41]))).
+    split; [reflexivity |].
+    split; [reflexivity |].
+    split; [apply simple_final_fields |].
+    split; [apply simple_cache_field_assignable |].
+    split.
+    + unfold simple_heap, simple_obj, simple_loc, simple_abs_fields.
+      constructor.
+      * unfold field_read.
+        exists (mkObj (mkruntime_type Imm_r simple_class)
+          [Int 41; Int (simple_derived [Int 41])]).
+        split; reflexivity.
+      * constructor.
+    + split.
+      * unfold field_read, simple_heap, simple_obj, simple_loc,
+          simple_cache_field.
+        exists (mkObj (mkruntime_type Imm_r simple_class)
+          [Int 41; Int (simple_derived [Int 41])]).
+        split; reflexivity.
+      * split; [reflexivity |].
+        unfold simple_derived. discriminate.
+Qed.
+
+Lemma simple_weak_two_duplicate_writes_execution :
+  weak_execution
+    simple_CT
+    simple_derived
+    simple_sc_initial_heap
+    [simple_weak_coherent_event; simple_weak_coherent_rewrite_event]
+    simple_sc_cache_written_heap.
+Proof.
+  eapply WE_Cons.
+  - apply simple_weak_accepts_coherent_cache_write.
+  - eapply WE_Cons.
+    + apply simple_sc_cache_written_heap_stable_write.
+    + apply WE_Nil.
+Qed.
+
+Lemma simple_initial_concurrent_cache_state :
+  concurrent_derived_cache_state
+    simple_CT
+    simple_sc_initial_heap
+    simple_loc
+    simple_class
+    simple_abs_fields
+    simple_cache_field
+    simple_derived.
+Proof.
+  exists (simple_obj (Int 41) (Int 0)).
+  split; [reflexivity |].
+  split; [reflexivity |].
+  exists [Int 41], (Int 0).
+  repeat split.
+  - apply simple_final_fields.
+  - apply simple_cache_field_assignable.
+  - apply simple_field_reads.
+  - apply simple_cache_read.
+  - left. reflexivity.
+Qed.
+
+Lemma simple_weak_two_duplicate_writes_preserve_cache_state :
+  concurrent_derived_cache_state
+    simple_CT
+    simple_sc_cache_written_heap
+    simple_loc
+    simple_class
+    simple_abs_fields
+    simple_cache_field
+    simple_derived.
+Proof.
+  eapply weak_execution_preserves_cache_state_for_target.
+  - apply simple_weak_two_duplicate_writes_execution.
+  - constructor.
+    + apply simple_weak_coherent_event_targets_cache.
+    + constructor.
+      * apply simple_weak_coherent_rewrite_event_targets_cache.
+      * constructor.
+  - apply simple_initial_concurrent_cache_state.
+Qed.
+
+Definition pair_left_field : var := 0.
+Definition pair_right_field : var := 1.
+Definition pair_cache_field : var := 2.
+Definition pair_root_class : class_name := 0.
+Definition pair_class : class_name := 1.
+
+Definition pair_left_field_def : field_def :=
+  {|
+    ftype :=
+      {|
+        assignability := Final;
+        mutability := Imm_f;
+        f_base_type := int_class_name
+      |};
+    fname := pair_left_field
+  |}.
+
+Definition pair_right_field_def : field_def :=
+  {|
+    ftype :=
+      {|
+        assignability := Final;
+        mutability := Imm_f;
+        f_base_type := int_class_name
+      |};
+    fname := pair_right_field
+  |}.
+
+Definition pair_cache_field_def : field_def :=
+  {|
+    ftype :=
+      {|
+        assignability := Assignable;
+        mutability := Imm_f;
+        f_base_type := int_class_name
+      |};
+    fname := pair_cache_field
+  |}.
+
+Definition pair_constructor : constructor_def :=
+  {|
+    csignature :=
+      {|
+        cqualifier := Imm_c;
+        cparams := []
+      |}
+  |}.
+
+Definition pair_root_class_def : class_def :=
+  {|
+    signature :=
+      {|
+        class_qualifier := Imm_c;
+        cname := pair_root_class;
+        super := None
+      |};
+    body :=
+      {|
+        fields := [];
+        constructor := pair_constructor;
+        methods := []
+      |}
+  |}.
+
+Definition pair_class_def : class_def :=
+  {|
+    signature :=
+      {|
+        class_qualifier := Imm_c;
+        cname := pair_class;
+        super := Some pair_root_class
+      |};
+    body :=
+      {|
+        fields := [pair_left_field_def; pair_right_field_def;
+          pair_cache_field_def];
+        constructor := pair_constructor;
+        methods := []
+      |}
+  |}.
+
+Definition pair_CT : class_table := [pair_root_class_def; pair_class_def].
+
+Definition pair_obj (left_v right_v cache_v : value) : Obj :=
+  mkObj
+    (mkruntime_type Imm_r pair_class)
+    [left_v; right_v; cache_v].
+
+Definition pair_heap (left_v right_v cache_v : value) : heap :=
+  [pair_obj left_v right_v cache_v].
+
+Definition pair_loc : Loc := 0.
+
+Definition pair_abs_fields : list var := [pair_left_field; pair_right_field].
+
+Definition pair_derived (vs : list value) : nat :=
+  match vs with
+  | [Int left_n; Int right_n] => left_n + right_n
+  | _ => 1
+  end.
+
+Definition pair_initial_heap : heap :=
+  pair_heap (Int 1) (Int 2) (Int 0).
+
+Definition pair_mixed_snapshot_event : weak_cache_write :=
+  mkWeakCacheWrite
+    pair_loc
+    pair_class
+    pair_abs_fields
+    pair_cache_field
+    [Int 1; Int 99]
+    (Int 0)
+    (pair_derived [Int 1; Int 99]).
+
+Definition pair_mixed_snapshot_heap : heap :=
+  update_field
+    pair_initial_heap
+    pair_loc
+    pair_cache_field
+    (Int (pair_derived [Int 1; Int 99])).
+
+Lemma pair_left_field_final :
+  final_field pair_CT pair_class pair_left_field.
+Proof.
+  unfold final_field, sf_assignability_rel, pair_CT, pair_class,
+    pair_left_field.
+  exists pair_left_field_def.
+  split.
+  - apply FL_Found with
+      (fields := [] ++ [pair_left_field_def; pair_right_field_def;
+        pair_cache_field_def]).
+    + eapply CF_Inherit.
+      * reflexivity.
+      * reflexivity.
+      * apply CF_Object with (def := pair_root_class_def); reflexivity.
+      * reflexivity.
+    + reflexivity.
+  - reflexivity.
+Qed.
+
+Lemma pair_right_field_final :
+  final_field pair_CT pair_class pair_right_field.
+Proof.
+  unfold final_field, sf_assignability_rel, pair_CT, pair_class,
+    pair_right_field.
+  exists pair_right_field_def.
+  split.
+  - apply FL_Found with
+      (fields := [] ++ [pair_left_field_def; pair_right_field_def;
+        pair_cache_field_def]).
+    + eapply CF_Inherit.
+      * reflexivity.
+      * reflexivity.
+      * apply CF_Object with (def := pair_root_class_def); reflexivity.
+      * reflexivity.
+    + reflexivity.
+  - reflexivity.
+Qed.
+
+Lemma pair_cache_field_assignable :
+  cache_field pair_CT pair_class pair_cache_field.
+Proof.
+  unfold cache_field, sf_assignability_rel, pair_CT, pair_class,
+    pair_cache_field.
+  exists pair_cache_field_def.
+  split.
+  - apply FL_Found with
+      (fields := [] ++ [pair_left_field_def; pair_right_field_def;
+        pair_cache_field_def]).
+    + eapply CF_Inherit.
+      * reflexivity.
+      * reflexivity.
+      * apply CF_Object with (def := pair_root_class_def); reflexivity.
+      * reflexivity.
+    + reflexivity.
+  - reflexivity.
+Qed.
+
+Lemma pair_final_fields :
+  final_fields pair_CT pair_class pair_abs_fields.
+Proof.
+  unfold final_fields, pair_abs_fields.
+  repeat constructor.
+  - apply pair_left_field_final.
+  - apply pair_right_field_final.
+Qed.
+
+Lemma pair_field_reads :
+  forall left_v right_v cache_v,
+    field_reads (pair_heap left_v right_v cache_v) pair_loc pair_abs_fields
+      [left_v; right_v].
+Proof.
+  intros left_v right_v cache_v.
+  unfold field_reads, pair_heap, pair_obj, pair_loc, pair_abs_fields.
+  repeat constructor.
+  - unfold field_read.
+    exists (mkObj (mkruntime_type Imm_r pair_class)
+      [left_v; right_v; cache_v]).
+    split; reflexivity.
+  - unfold field_read.
+    exists (mkObj (mkruntime_type Imm_r pair_class)
+      [left_v; right_v; cache_v]).
+    split; reflexivity.
+Qed.
+
+Lemma pair_cache_read :
+  forall left_v right_v cache_v,
+    field_read (pair_heap left_v right_v cache_v) pair_loc pair_cache_field
+      cache_v.
+Proof.
+  intros left_v right_v cache_v.
+  unfold field_read, pair_heap, pair_obj, pair_loc, pair_cache_field.
+  exists (mkObj (mkruntime_type Imm_r pair_class)
+    [left_v; right_v; cache_v]).
+  split; reflexivity.
+Qed.
+
+Lemma pair_mixed_snapshot_heap_not_protocol :
+  not
+    (derived_int_cache_protocol
+      pair_CT
+      pair_mixed_snapshot_heap
+      pair_loc
+      pair_class
+      pair_abs_fields
+      pair_cache_field
+      pair_derived).
+Proof.
+  intro Hprotocol.
+  destruct Hprotocol as
+    [abs_vals [cache_v [_ [_ [Hreads [Hcache_read Hcache_value]]]]]].
+  unfold pair_mixed_snapshot_heap, pair_initial_heap, pair_heap, pair_obj,
+    pair_loc, pair_abs_fields, pair_cache_field in *.
+  simpl in Hreads.
+  inversion Hreads as [|? ? left_v rest Hread_left Hreads_tail]; subst.
+  inversion Hreads_tail as [|? ? right_v rest_tail Hread_right Hreads_done];
+    subst.
+  inversion Hreads_done; subst.
+  destruct Hread_left as [o_left [Hobj_left Hfield_left]].
+  destruct Hread_right as [o_right [Hobj_right Hfield_right]].
+  simpl in Hobj_left, Hobj_right.
+  inversion Hobj_left; subst.
+  inversion Hobj_right; subst.
+  simpl in Hfield_left, Hfield_right.
+  inversion Hfield_left; subst.
+  inversion Hfield_right; subst.
+  destruct Hcache_read as [o_cache [Hobj_cache Hfield_cache]].
+  simpl in Hobj_cache.
+  inversion Hobj_cache; subst.
+  simpl in Hfield_cache.
+  inversion Hfield_cache; subst.
+  simpl in Hcache_value.
+  destruct Hcache_value as [Hunknown | Hknown].
+  - discriminate.
+  - destruct Hknown as [n [Hcache_eq [Hderived Hnz]]].
+    assert (Hn : n = pair_derived [Int 1; Int 99]).
+    { inversion Hcache_eq. reflexivity. }
+    simpl in Hderived.
+    simpl in Hn.
+    lia.
+Qed.
+
+Lemma pair_weak_rejects_mixed_snapshot :
+  weak_rejects_cache_transition
+    pair_CT
+    pair_initial_heap
+    pair_mixed_snapshot_heap
+    pair_derived
+    pair_mixed_snapshot_event.
+Proof.
+  eapply weak_rejects_protocol_break.
+  - reflexivity.
+  - apply pair_mixed_snapshot_heap_not_protocol.
+Qed.
+
+Lemma pair_weak_rejects_mixed_snapshot_execution :
+  weak_rejects_execution
+    pair_CT
+    pair_derived
+    pair_initial_heap
+    [pair_mixed_snapshot_event]
+    pair_mixed_snapshot_heap.
+Proof.
+  eapply weak_rejects_execution_at_head.
+  - reflexivity.
+  - apply pair_weak_rejects_mixed_snapshot.
+  - apply WCE_Nil.
+Qed.
